Removing references to generate_manifest from ManCompSoundness proofs.  Moved to files named *_Local.v

src/Manifest_Generator.v
@@ -141,95 +141,11 @@ Proof.
     try (destruct p1; break_if; congruence).
 Qed.
 
-Fixpoint add_to_list {A : Type} `{EqClass A} (l : list A) (v : A) : list A :=
-  match l with
-  | nil => v :: nil
-  | h :: t => if (eqb h v) then (h :: t) else h :: (add_to_list t v)
-  end.
 
-Fixpoint generate_manifest' (t : Term) (p : Plc) 
-    (m : Manifest) : Manifest :=
-  match t with
-  | asp a =>
-      (* Only update manifest of myself *)
-      if (eqb p m.(my_abstract_plc))
-      then
-        match a with
-        | NULL => m
-        | CPY => m
-        | ASPC _ _ (asp_paramsC aspid args targp targid) =>
-            {|
-              my_abstract_plc := m.(my_abstract_plc) ;
 
-              asps := add_to_list (m.(asps)) aspid ;
-              uuidPlcs := m.(uuidPlcs) ;
-              pubKeyPlcs := m.(pubKeyPlcs) ;
-              targetPlcs := add_to_list (m.(targetPlcs)) targp ;
-              policy := m.(policy) ;
-            |}
-        | SIG =>
-            {|
-              my_abstract_plc := m.(my_abstract_plc) ;
 
-              asps := add_to_list (m.(asps)) sig_aspid ;
-              uuidPlcs := m.(uuidPlcs) ;
-              pubKeyPlcs := m.(pubKeyPlcs) ;
-              targetPlcs := m.(targetPlcs) ;
-              policy := m.(policy) ;
-            |}
-        | HSH =>
-            {|
-              my_abstract_plc := m.(my_abstract_plc) ;
 
-              asps := add_to_list (m.(asps)) hsh_aspid ;
-              uuidPlcs := m.(uuidPlcs) ;
-              pubKeyPlcs := m.(pubKeyPlcs) ;
-              targetPlcs := m.(targetPlcs) ;
-              policy := m.(policy) ;
-            |}
-        | ENC p =>
-            {|
-              my_abstract_plc := m.(my_abstract_plc) ;
 
-              asps := add_to_list (m.(asps)) enc_aspid ;
-              uuidPlcs := m.(uuidPlcs) ;
-              pubKeyPlcs := add_to_list (m.(pubKeyPlcs)) p ;
-              targetPlcs := m.(targetPlcs) ;
-              policy := m.(policy) ;
-            |}
-        end
-      else m
-  | att p' t' =>
-      (* generate_manifest' t' p' *)
-      ({|
-        my_abstract_plc := m.(my_abstract_plc) ;
-
-        asps := m.(asps) ;
-        uuidPlcs := add_to_list (m.(uuidPlcs)) p' ;
-        pubKeyPlcs := m.(pubKeyPlcs) ;
-        targetPlcs := m.(targetPlcs) ;
-        policy := m.(policy) ;
-      |})
-  | lseq t1 t2 =>
-      generate_manifest' t2 p (generate_manifest' t1 p m)
-  | bseq _ t1 t2 =>
-      generate_manifest' t2 p (generate_manifest' t1 p m)
-  | bpar _ t1 t2 =>
-      generate_manifest' t2 p (generate_manifest' t1 p m)
-  end.
-
-Definition generate_manifest (t : Term) (p : Plc) :=
-  generate_manifest' t p (
-    {|
-      my_abstract_plc := p ;
-
-      asps := empty_Manifest.(asps) ;
-      uuidPlcs := empty_Manifest.(uuidPlcs) ;
-      pubKeyPlcs := empty_Manifest.(pubKeyPlcs) ;
-      targetPlcs := empty_Manifest.(targetPlcs) ;
-      policy := empty_Manifest.(policy) ;
-    |}
-  ).
 
 (*
 Fixpoint places' (t:Term) (ls:list Plc) : list Plc :=
