src/ManCompSoundness_Local.v
@@ -1,0 +1,3301 @@
+Require Import Manifest Manifest_Compiler Manifest_Generator AbstractedTypes
+  Maps Term_Defs List Cvm_St Cvm_Impl ErrorStMonad_Coq StructTactics 
+  Cvm_Monad EqClass Manifest_Admits Auto.
+Require Import Manifest_Generator_Facts Executable_Defs_Prop 
+  Executable_Facts_Dist Eqb_Evidence.
+
+Require Import Coq.Program.Tactics.
+
+Import ListNotations.
+
+(* Set Nested Proofs Allowed. *)
+
+
+(* map_get (minify_mapD Local_Plcs (fun _ : Plc => false)) p1 *)
+
+Fixpoint knowsOf_asps (tp : Plc) (p : Plc) (t : Term) : list ASP_ID :=
+  match t with
+  | asp a =>
+    if (eqb tp p)
+    then 
+      (match a with
+      | ASPC _ _ par =>
+          match par with
+          | asp_paramsC i _ targp targid => [i]
+          end
+      | SIG => [sig_aspid]
+      | HSH => [hsh_aspid]
+      | ENC p => [enc_aspid]
+      | _ => nil
+      end)
+    else nil
+  | att p' t' => knowsOf_asps tp p' t'
+  | lseq t1 t2 =>
+      knowsOf_asps tp p t1 ++ knowsOf_asps tp p t2
+  | bseq _ t1 t2 =>
+      knowsOf_asps tp p t1 ++ knowsOf_asps tp p t2
+  | bpar _ t1 t2 =>
+      knowsOf_asps tp p t1 ++ knowsOf_asps tp p t2
+  end.
+
+Fixpoint knowsOf_uuid' (tp : Plc) (p:Plc) (t:Term)  : list Plc :=
+  match t with
+  | asp a => nil
+  | att p' t' => 
+      if (eqb tp p)
+      then (* We are the top-level place, we need to know this *) 
+        p' :: knowsOf_uuid' tp p' t'
+      else knowsOf_uuid' tp p' t'
+  | lseq t1 t2 =>
+     knowsOf_uuid' tp p t1 ++ knowsOf_uuid' tp p t2
+  | bseq _ t1 t2 =>
+     knowsOf_uuid' tp p t1 ++ knowsOf_uuid' tp p t2
+  | bpar _ t1 t2 =>
+     knowsOf_uuid' tp p t1 ++ knowsOf_uuid' tp p t2
+  end.
+
+Fixpoint knowsOf_uuid'' (tp : Plc) (p:Plc) (t:Term)  : list Plc :=
+  match t with
+  | asp a => nil
+  | att p' t' => 
+      if (eqb tp p)
+      then (* We are the top-level place, we need to know this *) 
+        p' :: knowsOf_uuid'' p' p t'
+      else knowsOf_uuid'' p' p t'
+  | lseq t1 t2 =>
+     knowsOf_uuid'' tp p t1 ++ knowsOf_uuid'' tp p t2
+  | bseq _ t1 t2 =>
+     knowsOf_uuid'' tp p t1 ++ knowsOf_uuid'' tp p t2
+  | bpar _ t1 t2 =>
+     knowsOf_uuid'' tp p t1 ++ knowsOf_uuid'' tp p t2
+  end.
+
+Fixpoint mentioned_places (t : Term) : list Plc :=
+  match t with
+  | asp a => nil
+  | att p' t' => 
+      p' :: mentioned_places t'
+  | lseq t1 t2 =>
+      mentioned_places t1 ++ mentioned_places t2
+  | bseq _ t1 t2 =>
+      mentioned_places t1 ++ mentioned_places t2
+  | bpar _ t1 t2 =>
+      mentioned_places t1 ++ mentioned_places t2
+  end.
+
+Fixpoint knowsOf_pubkey' (tp : Plc) (p : Plc) (t : Term) : list ASP_ID :=
+  match t with
+  | asp a =>
+    match a with
+    | ENC p => if (eqb tp p) then [p] else nil
+    | _ => nil
+    end
+  | att p' t' => knowsOf_pubkey' tp p' t'
+  | lseq t1 t2 =>
+      knowsOf_pubkey' tp p t1 ++ knowsOf_pubkey' tp p t2
+  | bseq _ t1 t2 =>
+      knowsOf_pubkey' tp p t1 ++ knowsOf_pubkey' tp p t2
+  | bpar _ t1 t2 =>
+      knowsOf_pubkey' tp p t1 ++ knowsOf_pubkey' tp p t2
+  end.
+
+Fixpoint static_executable_manifest (t : Term) (m : Manifest) : Prop :=
+  match t with
+  | asp a => 
+      match a with
+      | ASPC _ _ par =>
+          match par with
+          | asp_paramsC i _ targp targid => 
+              In i (asps m)
+          end
+      | SIG => In sig_aspid (asps m)
+      | HSH => In hsh_aspid (asps m)
+      | ENC p => In enc_aspid (asps m) /\ In p (pubKeyPlcs m)
+      | NULL => True
+      | CPY => True 
+      end
+  | att p' t => In p' (uuidPlcs m)
+  | lseq t1 t2 => static_executable_manifest t1 m /\ static_executable_manifest t2 m
+  | bseq _ t1 t2 => static_executable_manifest t1 m /\ static_executable_manifest t2 m
+  | bpar _ t1 t2 => static_executable_manifest t1 m /\ static_executable_manifest t2 m
+  end.
+
+Ltac grind :=
+  repeat (try break_match; simpl in *; intuition; subst; eauto; try congruence);
+  repeat find_injection; subst;
+  simpl in *; intuition; eauto.
+
+Ltac breq l r :=
+  let E := fresh "Heq" in
+  destruct (eqb l r) eqn:E;
+  try rewrite E in *;
+  try (rewrite eqb_leibniz in *; subst; simpl in *; intuition; eauto; try congruence);
+  try (rewrite eqb_refl in *; subst; simpl in *; intuition; eauto; try congruence);
+  try (assert (l <> r) by (intros HC; rewrite <- eqb_leibniz in *; congruence)).
+
+Ltac unf :=
+  repeat (unfold asp_manifest_generator,
+    at_manifest_generator, knowsof_manifest_update,
+    asp_manifest_update, manifest_update_env,
+    aspid_manifest_update, update_manifest_policy_targ,
+    empty_Manifest in *
+  ); simpl in *; try (intuition; eauto; congruence).
+(* 
+
+Theorem man_gen_only_available_if_known : forall t p backEnv envM p',
+  map_get backEnv p' = None ->
+  manifest_generator' p t backEnv = envM ->
+  ((exists man, map_get envM p' = Some man) <-> In p' (knowsOf_uuid' p p' t)).
+Proof.
+  induction t; simpl in *; intuition; eauto; subst.
+  - unfold asp_manifest_generator, manifest_update_env, 
+      asp_manifest_update, aspid_manifest_update, update_manifest_policy_targ,
+      pubkey_manifest_update in *; simpl in *; destruct H1.
+    destruct a; simpl in *;
+    break_match; subst;
+    breq p p';
+    erewrite mapC_get_distinct_keys_from_set in H; intuition; eauto; try congruence.
+  - unfold asp_manifest_generator, manifest_update_env, 
+      asp_manifest_update, aspid_manifest_update, update_manifest_policy_targ,
+      pubkey_manifest_update in *; simpl in *.
+    destruct a; simpl in *;
+    repeat break_match; subst; simpl in *; eauto; try congruence;
+    try rewrite mapC_get_works; eexists; eauto.
+  - breq p0 p'.
+    unfold at_manifest_generator, manifest_update_env, knowsof_manifest_update in *;
+    simpl in *.
+    destruct (manifest_generator' p t
+            (map_set backEnv p0
+               (let
+                '{|
+                   my_abstract_plc := oldPlc;
+                   asps := oldasps;
+                   uuidPlcs := oldKnowsOf;
+                   pubKeyPlcs := oldContext;
+                   targetPlcs := oldTargets;
+                   policy := oldPolicy
+                 |} := match map_get backEnv p0 with
+                       | Some mm => mm
+                       | None => empty_Manifest
+                       end in
+                 {|
+                   my_abstract_plc := oldPlc;
+                   asps := oldasps;
+                   uuidPlcs := p :: oldKnowsOf;
+                   pubKeyPlcs := oldContext;
+                   targetPlcs := oldTargets;
+                   policy := oldPolicy
+                 |}))) eqn:E;
+    try (exfalso; eapply manifest_generator_never_empty; eauto; fail).
+    repeat break_match; simpl in *; eauto;
+    repeat break_match; simpl in *.
+    * destruct H1; repeat find_injection; simpl in *.
+      rewrite eqb_leibniz in *; subst.
+      assert (map_get (map_set backEnv p0
+         {|
+           my_abstract_plc := my_abstract_plc;
+           asps := asps;
+           uuidPlcs := p :: uuidPlcs;
+           pubKeyPlcs := pubKeyPlcs;
+           targetPlcs := targetPlcs;
+           policy := policy
+         |}) p' = None). admit.
+      pose proof (IHt _ _ _ _ H1 E).
+      assert (exists man, map_get ((p',x) :: e) p' = Some man). admit.
+      rewrite H2 in H3; intuition; eauto; subst.
+
+Theorem man_gen_only_available_if_known : forall t p backEnv envM p',
+  map_get backEnv p' = None ->
+  manifest_generator' p t backEnv = envM ->
+  ((exists man, map_get envM p' = Some man) <-> (In p' (knowsOf_uuid' p p' t) \/ p = p')).
+Proof.
+  induction t; simpl in *; intuition; eauto; subst.
+  - unfold asp_manifest_generator, manifest_update_env, 
+      asp_manifest_update, aspid_manifest_update, update_manifest_policy_targ,
+      pubkey_manifest_update in *; simpl in *. destruct H1.
+    destruct a; simpl in *;
+    break_match; subst;
+    breq p p';
+    erewrite mapC_get_distinct_keys_from_set in H; intuition; eauto; try congruence.
+  - unfold asp_manifest_generator, manifest_update_env, 
+      asp_manifest_update, aspid_manifest_update, update_manifest_policy_targ,
+      pubkey_manifest_update in *; simpl in *.
+    destruct a; simpl in *;
+    repeat break_match; subst; simpl in *; eauto; try congruence;
+    try rewrite mapC_get_works; eexists; eauto.
+  - breq p0 p'.
+    unfold at_manifest_generator, manifest_update_env, knowsof_manifest_update in *;
+    simpl in *.
+    destruct (manifest_generator' p t
+            (map_set backEnv p0
+               (let
+                '{|
+                   my_abstract_plc := oldPlc;
+                   asps := oldasps;
+                   uuidPlcs := oldKnowsOf;
+                   pubKeyPlcs := oldContext;
+                   targetPlcs := oldTargets;
+                   policy := oldPolicy
+                 |} := match map_get backEnv p0 with
+                       | Some mm => mm
+                       | None => empty_Manifest
+                       end in
+                 {|
+                   my_abstract_plc := oldPlc;
+                   asps := oldasps;
+                   uuidPlcs := p :: oldKnowsOf;
+                   pubKeyPlcs := oldContext;
+                   targetPlcs := oldTargets;
+                   policy := oldPolicy
+                 |}))) eqn:E;
+    try (exfalso; eapply manifest_generator_never_empty; eauto; fail).
+    repeat break_match; simpl in *; eauto;
+    repeat break_match; simpl in *.
+    * destruct H1; repeat find_injection; simpl in *.
+      rewrite eqb_leibniz in *; subst.
+      assert (map_get (map_set backEnv p0
+         {|
+           my_abstract_plc := my_abstract_plc;
+           asps := asps;
+           uuidPlcs := p :: uuidPlcs;
+           pubKeyPlcs := pubKeyPlcs;
+           targetPlcs := targetPlcs;
+           policy := policy
+         |}) p' = None). admit.
+      pose proof (IHt _ _ _ _ H1 E).
+      assert (exists man, map_get ((p',x) :: e) p' = Some man). admit.
+      rewrite H2 in H3; intuition; eauto; subst. *)
+
+    
+
+(* Theorem manifest_generator_impl_static_executable_manifest : forall t p backEnv envM,
+  (forall p' man,
+    map_get backEnv p' = Some man ->
+    static_executable_manifest t man) ->
+  manifest_generator' p t backEnv = envM ->
+  (forall p' man,
+    map_get envM p' = Some man ->
+    static_executable_manifest t man
+  ).
+Proof.
+  induction t; simpl in *; intuition; eauto.
+  - destruct a; simpl in *; intuition; eauto.
+    * destruct a; simpl in *; eauto.
+      unfold asp_manifest_generator, manifest_update_env, 
+        asp_manifest_update, aspid_manifest_update, 
+        update_manifest_policy_targ in *; simpl in *;
+      repeat break_match; simpl in *;
+      repeat find_injection.
+      ** eapply H in Heqo; simpl in *.
+  
+Qed. *)
+
+
+(* Theorem manifest_generator_works : forall t p backEnv envM,
+  manifest_generator' p t backEnv = envM ->
+  forall p' absMan,
+    map_get envM p' = Some absMan ->
+    ((forall (a : ASP_ID), In a (knowsOf_asps p p' t) -> In a (asps absMan)) /\ 
+     (forall (u : Plc), In u (knowsOf_uuid' p p' t) -> In u (uuidPlcs absMan)) /\
+     (forall (u : Plc), In u (knowsOf_pubkey' p p' t) -> In u (pubKeyPlcs absMan))).
+Proof.
+  intros t p stEnv.
+  pose proof (manifest_generator_executability_static' t p stEnv).
+  generalizeEverythingElse t.
+  induction t; simpl in *; intros.
+  - destruct a; simpl in *;
+    repeat break_match; simpl in *; intuition; eauto;
+    subst.
+    unfold canRunAsp_Env in *.
+
+
+  simpl in *.
+
+  induction t; simpl in *; intros.
+  - repeat break_match; simpl in *; intuition; subst; eauto; 
+    try congruence; unfold canRunAsp_Env in *; simpl in *; eauto;
+    try break_if; try (rewrite eqb_leibniz in *; subst; eauto); admit.
+  - eapply IHt in H as IH; simpl in *; intuition; eauto;
+    break_if; eauto; clear IHt; rewrite <- H in H0. clear H.
+    rewrite eqb_leibniz in *.
+    rewrite Heqb in *; clear Heqb; eauto; simpl in *;
+    intuition; rewrite H in *. clear H.
+    unfold at_manifest_generator, manifest_update_env, knowsof_manifest_update 
+      in *; repeat break_match; subst; simpl in *; intuition; eauto;
+    pose proof (man_gen_map_getter t u p'
+             {|
+               my_abstract_plc := my_abstract_plc;
+               asps := asps;
+               uuidPlcs := u :: uuidPlcs;
+               pubKeyPlcs := pubKeyPlcs;
+               targetPlcs := targetPlcs;
+               policy := policy
+             |} backEnv); destruct H; intuition; simpl in *; 
+    find_rewrite; find_injection; eauto.
+  - 
+    destruct (manifest_generator' p t1 backEnv) eqn:E1;
+    try (exfalso; eapply manifest_generator_never_empty; eauto; fail);
+    destruct (map_get (manifest_generator' p t1 backEnv) p') eqn:E2.
+    * rewrite E1 in E2;
+      pose proof (IHt1 p backEnv (p0 :: e) E1 _ _ E2).
+      pose proof (IHt2 p (p0 :: e) envM H _ _ H0);
+      intuition; rewrite in_app_iff in *; intuition; eauto;
+      clear IHt1 IHt2; admit.
+    * 
+    pose proof (man_gen_map_getter).
+    intuition; rewrite in_app_iff in *; intuition.
+    * destruct (manifest_generator' p t1 backEnv) eqn:E1;
+      try (exfalso; eapply manifest_generator_never_empty; eauto; fail);
+      destruct p0; simpl in *.
+      pose proof (IHt1 _ _ _ E1 p'); simpl in *;
+      break_if; try (rewrite eqb_leibniz in *; subst; intuition; eauto).
+      admit.
+      pose proof (man_gen_doesnt_kill_info).
+    pose proof (IHt1 _ _ _ E1). clear IHt1 E1.
+    destruct p0.
+    destruct (manifest_generator' p t2 ((p0, m) :: e)) eqn:E2;
+    try (exfalso; eapply manifest_generator_never_empty; eauto; fail).
+    pose proof (IHt2 _ _ _ E2); destruct p1; simpl in *. clear IHt2; simpl in *; subst.
+    simpl in *.
+    break_if; try (rewrite eqb_leibniz in *; subst; eauto; find_injection).
+    * intuition; eauto; rewrite in_app_iff in *; intuition; eauto.
+    simpl in *; intuition; eauto.
+    * eapply IHt1 in E1 as E'.
+    eapply IHt1 in E1.
+    destruct H; eapply IHt1 in H; eapply IHt2 in H1; eauto;
+    intuition; rewrite in_app_iff in *; intuition; eauto.
+  - destruct H; eapply IHt1 in H; eapply IHt2 in H1; eauto;
+    intuition; rewrite in_app_iff in *; intuition; eauto.
+  - destruct H; eapply IHt1 in H; eapply IHt2 in H1; eauto;
+    intuition; rewrite in_app_iff in *; intuition; eauto.
+Qed. *)
+
+
+Ltac cunf :=
+  repeat (unfold asp_manifest_generator,
+    asp_manifest_update,
+    aspid_manifest_update,
+    at_manifest_generator,
+    manifest_update_env,
+    knowsof_manifest_update,
+    update_manifest_policy_targ,
+    pubkey_manifest_update,
+    map_set;
+  simpl in *; eauto);
+  repeat break_match;
+  repeat find_injection;
+  subst;
+  repeat find_inversion;
+  try congruence;
+  simpl in *;
+  eauto.
+(* 
+Lemma man_gen_map_getter : forall t u preEnv p st postEnv,
+  map_get preEnv p = None ->
+  exists st', 
+    (map_get (manifest_generator' u t (preEnv ++ (p, st) :: postEnv)) p = Some st') /\
+    (forall x, In x st.(uuidPlcs) -> In x st'.(uuidPlcs)) /\
+    (forall x, In x st.(asps) -> In x st'.(asps)) /\
+    (forall x, In x st.(pubKeyPlcs) -> In x st'.(pubKeyPlcs)).
+Proof.
+
+  induction t; simpl in *; intuition; eauto.
+  - break_if.
+    * rewrite eqb_leibniz in *; subst;
+      break_match; try (edestruct @map_sandwich_not_none; eauto; fail);
+      eapply map_app_unfolder in Heqo; subst; eauto;
+      eexists; intuition; cunf.
+    * destruct (map_has_buried preEnv p st postEnv);
+      pose proof (map_app_unfolder preEnv p st postEnv _ H0 H); subst;
+      eexists; intuition; cunf.
+  - cunf.
+    * pose proof (IHt p ((u,
+         {|
+           my_abstract_plc := my_abstract_plc;
+           asps := asps;
+           uuidPlcs := p :: uuidPlcs;
+           pubKeyPlcs := pubKeyPlcs;
+           targetPlcs := targetPlcs;
+           policy := policy
+         |}) :: preEnv) p0 ).
+    cunf; eexists; intuition; eauto.
+      break_match.
+      admit.
+      
+      exfalso. eapply map_sandwich_not_none; eauto.
+      admit.
+      break_match; eexists; intuition; cunf; destruct a; 
+      pose proof (map_app_unfolder preEnv u st postEnv _ Heqo H); subst. *)
+
+(* Definition knowsOf_pubkey (p : Plc) (t : Term) : list ASP_ID :=
+  p :: (knowsOf_pubkey' p t). *)
+(* Lemma man_gen_doesnt_kill_info : forall t u p st absMan preEnv postEnv,
+  map_get 
+    (manifest_generator' u t
+      (preEnv ++ (p, st) :: postEnv)) p = Some absMan ->
+  map_get preEnv p = None ->
+  forall x,
+  In x (st.(uuidPlcs)) ->
+  In x (absMan.(uuidPlcs)).
+Proof.
+  induction t; simpl in *; intuition; eauto.
+  - break_if; unfold asp_manifest_update, aspid_manifest_update,
+      update_manifest_policy_targ, pubkey_manifest_update in *; simpl in *;
+    repeat break_match; repeat find_injection; simpl in *; eauto; try congruence;
+    try (rewrite eqb_leibniz in *; subst; simpl in *; eauto);
+    try (eapply map_app_unfolder in Heqo; subst; eauto; fail);
+    try (eapply map_sandwich_not_none in Heqo; exfalso; eauto; fail).
+    * eapply map_app_unfolder in H; subst; simpl in *; eauto.
+  - unfold at_manifest_generator, manifest_update_env, knowsof_manifest_update, map_set in *.
+    break_match.
+    destruct (eqb u p0) eqn:E.
+    * rewrite eqb_leibniz in *; subst.
+      pose proof (IHt p p0 {|
+             my_abstract_plc := my_abstract_plc;
+             asps := asps;
+             uuidPlcs := p :: uuidPlcs;
+             pubKeyPlcs := pubKeyPlcs;
+             targetPlcs := targetPlcs;
+             policy := policy
+           |} absMan nil (preEnv ++ (p0, st) :: postEnv)); simpl in *.
+      break_match; subst; simpl in *; intuition; eauto.
+      ** eapply map_app_unfolder in Heqo; eauto; destruct st; find_injection; eauto.
+      ** eapply map_sandwich_not_none in Heqo; exfalso; eauto.
+    * pose proof (IHt p p0 st absMan ((u,
+           {|
+             my_abstract_plc := my_abstract_plc;
+             asps := asps;
+             uuidPlcs := p :: uuidPlcs;
+             pubKeyPlcs := pubKeyPlcs;
+             targetPlcs := targetPlcs;
+             policy := policy
+           |}) :: preEnv) postEnv). rewrite app_comm_cons in *;
+           intuition; eapply H3; eauto.
+      simpl in *. rewrite eqb_symm. rewrite E; eauto.
+  - destruct (manifest_generator' u t1 (preEnv ++ (p, st) :: postEnv)) eqn:E;
+    try (exfalso; eapply manifest_generator_never_empty; eauto; fail);
+    destruct p0.
+    destruct (map_get ((p0, m) :: e) p) eqn:E1.
+    destruct (manifest_generator' u t2 (p0 :: e))
+
+    eapply (IHt1 u p st absMan preEnv postEnv); eauto.
+    destruct (manifest_generator' u t1 (preEnv ++ (p, st) :: postEnv)) eqn:E;
+    
+
+
+    (* * pose proof (IHt p p0 {|
+             my_abstract_plc := my_abstract_plc;
+             asps := asps;
+             uuidPlcs := p :: uuidPlcs;
+             pubKeyPlcs := pubKeyPlcs;
+             targetPlcs := targetPlcs;
+             policy := policy
+           |} absMan nil (preEnv ++ (p0, st) :: postEnv)); simpl in *;
+      eapply H2; eauto.
+      break_match; subst; simpl in *; intuition; eauto.
+      ** eapply map_app_unfolder in Heqo; eauto; destruct st; find_injection; eauto.
+      ** eapply map_sandwich_not_none in Heqo; exfalso; eauto.
+      intuition; eapply H2; intuition; eauto.
+     rewrite app_comm_cons in *; eapply IHt in H; eauto.
+    simpl in *.
+    pose proof (IHt p p0 st absMan ((u,
+           {|
+             my_abstract_plc := my_abstract_plc;
+             asps := asps;
+             uuidPlcs := p :: uuidPlcs;
+             pubKeyPlcs := pubKeyPlcs;
+             targetPlcs := targetPlcs;
+             policy := policy
+           |}) :: preEnv ) ).
+    rewrite <- H.
+    pose proof (IHt p u {|
+             my_abstract_plc := my_abstract_plc;
+             asps := asps;
+             uuidPlcs := p :: uuidPlcs;
+             pubKeyPlcs := pubKeyPlcs;
+             targetPlcs := targetPlcs;
+             policy := policy
+           |} absMan ((p0, st) :: backEnv)); intuition.
+    eapply IHt in H.
+    repeat find_injection; try find_contradiction. *)
+Admitted. *)
+
+(* Global Hint Resolve man_gen_doesnt_kill_info : core. *)
+
+(* Theorem executable_impl_precond : forall t p backEnv envM,
+  manifest_generator' p t backEnv = envM ->
+  (forall p' absMan,
+    map_get envM p' = Some absMan ->
+    ((forall (a : ASP_ID), In a (knowsOf_asps p p' t) -> In a (asps absMan)) /\ 
+     (forall (u : Plc), In u (knowsOf_uuid' p p' t) -> In u (uuidPlcs absMan)) /\
+     (forall (u : Plc), In u (knowsOf_pubkey' p p' t) -> In u (pubKeyPlcs absMan)))
+  ).
+Proof.
+  induction t; simpl in *; intros.
+  - repeat break_match; simpl in *; intuition; subst; eauto; 
+    try congruence; unfold canRunAsp_Env in *; simpl in *;
+    break_if; try (rewrite eqb_leibniz in *; subst; eauto);
+    admit.
+  - eapply IHt in H as IH; simpl in *; intuition; eauto;
+    break_if; eauto; clear IHt; rewrite <- H in H0. clear H.
+    rewrite eqb_leibniz in *.
+    rewrite Heqb in *; clear Heqb; eauto; simpl in *;
+    intuition; rewrite H in *. clear H.
+    unfold at_manifest_generator, manifest_update_env, knowsof_manifest_update,
+      map_set in *; repeat break_match; subst; simpl in *; intuition; eauto;
+    eapply man_gen_doesnt_kill_info with (preEnv := nil); eauto; simpl in *; eauto.
+  - intuition; rewrite in_app_iff in *; intuition.
+    * destruct (manifest_generator' p t1 backEnv) eqn:E1;
+      try (exfalso; eapply manifest_generator_never_empty; eauto; fail);
+      destruct p0; simpl in *.
+      pose proof (IHt1 _ _ _ E1 p'); simpl in *;
+      break_if; try (rewrite eqb_leibniz in *; subst; intuition; eauto).
+      pose proof (man_gen_doesnt_kill_info).
+    pose proof (IHt1 _ _ _ E1). clear IHt1 E1.
+    destruct p0.
+    destruct (manifest_generator' p t2 ((p0, m) :: e)) eqn:E2;
+    try (exfalso; eapply manifest_generator_never_empty; eauto; fail).
+    pose proof (IHt2 _ _ _ E2); destruct p1; simpl in *. clear IHt2; simpl in *; subst.
+    simpl in *.
+    break_if; try (rewrite eqb_leibniz in *; subst; eauto; find_injection).
+    * intuition; eauto; rewrite in_app_iff in *; intuition; eauto.
+    simpl in *; intuition; eauto.
+    * eapply IHt1 in E1 as E'.
+    eapply IHt1 in E1.
+    destruct H; eapply IHt1 in H; eapply IHt2 in H1; eauto;
+    intuition; rewrite in_app_iff in *; intuition; eauto.
+  - destruct H; eapply IHt1 in H; eapply IHt2 in H1; eauto;
+    intuition; rewrite in_app_iff in *; intuition; eauto.
+  - destruct H; eapply IHt1 in H; eapply IHt2 in H1; eauto;
+    intuition; rewrite in_app_iff in *; intuition; eauto.
+Admitted. *)
+
+Definition lib_supports_manifest (al : AM_Library) (am : Manifest) : Prop :=
+  (forall (a : ASP_ID), In a am.(asps) -> exists cb, Maps.map_get al.(Local_ASPS) a = Some cb) /\
+  (forall (up : Plc), In up am.(uuidPlcs) -> exists b, Maps.map_get al.(Local_Plcs) up = Some b) /\
+  (forall (pkp : Plc), In pkp am.(pubKeyPlcs) -> exists b, Maps.map_get al.(Local_PubKeys) pkp = Some b).
+
+Ltac unfolds :=
+  (* repeat monad_unfold; *)
+  repeat unfold manifest_generator, manifest_compiler, generate_ASP_dispatcher, 
+    generate_Plc_dispatcher, generate_PubKey_dispatcher,
+    generate_UUID_dispatcher, lib_supports_manifest, aspid_manifest_update,
+    sig_params, hsh_params, enc_params in *;
+  simpl in *; 
+  repeat (match goal with
+      | x : cvm_st |- _ => destruct x
+      | x : AM_Config |- _ => destruct x
+      | x : AM_Library |- _ => destruct x
+      | x : CallBackErrors |- _ => destruct x
+  end; simpl in *; eauto);
+  intuition.
+
+Theorem man_gen_aspid_in : forall a m,
+  In a (asps (aspid_manifest_update a m)).
+Proof.
+  induction m; simpl in *; eauto.
+Qed.
+
+
+
+(* Lemma stupid_map_killer : forall a Local_ASPS st_pl st_ev p t m l d,
+  (exists cb : CakeML_ASPCallback CallBackErrors, map_get Local_ASPS a = Some cb) ->
+  (match
+      map_get
+        (minify_mapC Local_ASPS
+            (fun x : ASP_ID =>
+            if
+              in_dec (EqClass_impl_DecEq ASP_ID) x (asps (aspid_manifest_update a (update_manifest_policy_targ p t m)))
+            then true
+            else false)) a
+        with
+        | Some cb =>
+            match cb (asp_paramsC a l p t) st_pl (encodeEvRaw (get_bits st_ev)) (get_bits st_ev) with
+            | errC c => match c with
+                        | messageLift _ => errC Runtime
+                        end
+            | resultC r => resultC r
+            end
+        | None => errC Unavailable
+        end = errC d) ->
+  d = Runtime.
+Proof.
+  destruct d; eauto; intros; repeat break_match; 
+  try congruence; clear H0.
+  destruct H; pose proof man_gen_aspid_in; eauto.
+  pose proof (H0 a). clear H0.
+  assert (Some x = None). {
+    rewrite <- H, <- Heqo.
+    clear Heqo H st_pl st_ev x l.
+    induction Local_ASPS; simpl in *; eauto.
+    rewrite IHLocal_ASPS. clear IHLocal_ASPS.
+    simpl in *.
+    destruct a0, (eqb a a0) eqn:E; simpl in *; eauto;
+    try (rewrite eqb_leibniz in E; subst; eauto).
+    - destruct (in_dec (EqClass_impl_DecEq ASP_ID) a0 (asps (aspid_manifest_update a0 (update_manifest_policy_targ p t m)))); simpl in *; try rewrite eqb_refl in *; eauto; try (pose proof (H1 (update_manifest_policy_targ p t m))); try congruence.
+    - destruct (in_dec (EqClass_impl_DecEq ASP_ID) a0 (asps (aspid_manifest_update a (update_manifest_policy_targ p t m)))); simpl in *; eauto; rewrite E; eauto.
+  }
+  congruence.
+Qed.
+
+
+Global Hint Resolve stupid_map_killer : core. *)
+Global Hint Resolve man_gen_aspid_in : core.
+
+(* 
+Lemma generated_uuid_plcs_not_none : forall (l : MapD Plc UUID) (p : Plc) t p0 backEnv p' absMan,
+  (map_get (manifest_generator' p t (at_manifest_generator p0 p backEnv)) p' = Some absMan) ->
+  (forall up : Plc, In up (uuidPlcs absMan) -> exists b : UUID, map_get l up = Some b) ->
+  (map_get (minify_mapD l 
+    (fun x : Plc => if in_dec (EqClass_impl_DecEq Plc) x (uuidPlcs absMan) then true else false)) p = None) ->
+  False.
+Proof.
+  induction l; simpl in *; intuition; eauto.
+  - admit.
+  - repeat (break_if; simpl in *; eauto; try congruence).
+    * admit.
+    * 
+    * pose proof (IHl _ _ _ _ _ _ H).
+      eapply IHl; eauto; intros.
+      destruct (H0 _ H2); break_if; eauto; invc H3.
+      rewrite eqb_leibniz in *; subst. *)
+
+Theorem filter_resolver : forall {A B} `{EqClass A} (m : MapC A B) a (filt : A -> bool),
+  (exists x, map_get m a = Some x) ->
+  filt a = true ->
+  exists x, map_get (minify_mapC m filt) a = Some x.
+Proof.
+  induction m; intuition; simpl in *;
+  destruct (eqb a a0) eqn:E.
+  - rewrite eqb_leibniz in E; subst. rewrite H1; simpl in *; rewrite eqb_refl; eauto.
+  - repeat break_match; simpl in *; 
+    try (pose proof eqb_symm; congruence);
+    simpl in *; eauto.
+    rewrite eqb_symm; rewrite E; eauto.
+Qed.
+
+
+Theorem filter_resolver_mapd : forall {A B} `{EqClass A, EqClass B} (m : MapC A B) a (filt : A -> bool),
+  (exists x, map_get m a = Some x) ->
+  filt a = true ->
+  exists x, map_get (minify_mapD m filt) a = Some x.
+Proof.
+  induction m; intuition; simpl in *;
+  destruct (eqb a a0) eqn:E.
+  - rewrite eqb_leibniz in E; subst; destruct H1; simpl in *; 
+    repeat find_injection; rewrite H2; simpl in *; rewrite eqb_refl; eauto.
+  - repeat break_match; simpl in *; 
+    try (pose proof eqb_symm; congruence);
+    simpl in *; eauto;
+    repeat (find_rewrite; intuition; eauto; try congruence).
+    rewrite eqb_symm in E; congruence.
+Qed.
+
+Global Hint Resolve filter_resolver : core.
+Global Hint Resolve filter_resolver_mapd : core.
+
+Lemma in_dec_helper : forall {A B} `{EqClass A} X l l' a (c : B),
+  map_get (minify_mapC l (fun x : A => if in_dec X x l' then true else false)) a = Some c ->
+  In a l'.
+Proof.
+  induction l; simpl in *; intuition; try congruence;
+  repeat break_if; eauto; simpl in *; 
+  repeat break_if; eauto; try rewrite eqb_leibniz in Heqb1; 
+  subst; eauto; congruence.
+Qed.
+
+Global Hint Resolve filter_resolver : core.
+
+Require Import Helpers_CvmSemantics.
+
+(* Lemma manifest_compiled_am_config_plcCb_only_unavailable : forall t st st' p, *)
+
+(* Theorem man_gen_subterm : forall (t : Term) getPl backEnv p absMan,
+  p <> getPl ->
+  map_get backEnv getPl = None ->
+  map_get (manifest_generator' p t backEnv) getPl = Some absMan ->
+  In p (knowsOf_uuid' p getPl t).
+Proof.
+  induction t; intuition; try (simpl in *; eauto; fail).
+  - unfold asp_manifest_generator, manifest_update_env, 
+      asp_manifest_update, aspid_manifest_update, update_manifest_policy_targ in *;
+    simpl in *.
+    eapply (map_set_unfolder _ getPl p); [eauto | | eapply H1 ].
+    erewrite map_get_none_iff_not_some; intros. 
+    eapply (map_set_unfolder _ getPl); eauto.
+  - admit.
+  - simpl in *. rewrite in_app_iff.
+    destruct (manifest_generator' p t1 backEnv) eqn:E1;
+    try (exfalso; eapply manifest_generator_never_empty; eauto; fail);
+    destruct (manifest_generator' p t2 (p0 :: e)) eqn:E2;
+    try (exfalso; eapply manifest_generator_never_empty; eauto; fail);
+    destruct (map_get (p0 :: e) getPl) eqn:E3.
+    * left; eapply IHt1; eauto; find_rewrite; eauto.
+    * right; eapply IHt2; eauto; find_rewrite; eauto.
+  - simpl in *. rewrite in_app_iff.
+    destruct (manifest_generator' p t1 backEnv) eqn:E1;
+    try (exfalso; eapply manifest_generator_never_empty; eauto; fail);
+    destruct (manifest_generator' p t2 (p0 :: e)) eqn:E2;
+    try (exfalso; eapply manifest_generator_never_empty; eauto; fail);
+    destruct (map_get (p0 :: e) getPl) eqn:E3.
+    * left; eapply IHt1; eauto; find_rewrite; eauto.
+    * right; eapply IHt2; eauto; find_rewrite; eauto.
+  - simpl in *. rewrite in_app_iff.
+    destruct (manifest_generator' p t1 backEnv) eqn:E1;
+    try (exfalso; eapply manifest_generator_never_empty; eauto; fail);
+    destruct (manifest_generator' p t2 (p0 :: e)) eqn:E2;
+    try (exfalso; eapply manifest_generator_never_empty; eauto; fail);
+    destruct (map_get (p0 :: e) getPl) eqn:E3.
+    * left; eapply IHt1; eauto; find_rewrite; eauto.
+    * right; eapply IHt2; eauto; find_rewrite; eauto.
+Admitted. *)
+
+Lemma callbacks_work_asps : forall absMan amLib amConf,
+  lib_supports_manifest amLib absMan ->
+  manifest_compiler absMan amLib = amConf ->
+  (forall x, In x absMan.(asps) -> 
+    forall l p t p' ev ev' res,
+      aspCb amConf (asp_paramsC x l p t) p' ev ev' = res ->
+      res = errC Runtime \/ exists r, res = resultC r
+  ).
+Proof.
+  induction absMan; simpl in *; intuition;
+  destruct res; eauto; destruct d; eauto.
+  destruct amConf; simpl in *;
+  destruct amLib; simpl in *.
+  unfold manifest_compiler in H0; repeat find_injection;
+  simpl in *.
+  repeat break_match; try congruence.
+  unfold lib_supports_manifest in *; simpl in *;
+  intuition.
+  pose proof (H0 _ H1).
+  assert ((fun x : ASP_ID =>
+             if in_dec (EqClass_impl_DecEq ASP_ID) x asps
+             then true
+             else false) x = true).
+  repeat break_match; eauto.
+  pose proof (filter_resolver _ _ ((fun x : ASP_ID =>
+             if in_dec (EqClass_impl_DecEq ASP_ID) x asps
+             then true
+             else false)) H3 H5).
+  destruct H6. 
+  assert (Some x0 = None). 
+  rewrite <- H6. rewrite <- Heqo; eauto.
+  congruence.
+Qed.
+
+Lemma add_to_list_works : forall {A} `{EqClass A} (l : list A) x,
+  In x (add_to_list l x).
+Proof.
+  induction l; simpl in *; intuition; eauto;
+  break_match; simpl in *; eauto.
+  - rewrite eqb_leibniz in *; subst; eauto.
+Qed.
+
+Local Hint Resolve add_to_list_works : core.
+
+Lemma never_change_am_conf : forall t st res st',
+  build_cvm (copland_compile t) st = (res, st') ->
+  st_AM_config st = st_AM_config st'.
+Proof.
+  induction t; simpl in *; 
+  subst; simpl in *; try rewrite eqb_refl in *;
+  repeat (
+    try break_match;
+    try monad_unfold;
+    try break_match
+    try find_injection;
+    try find_contradiction;
+    try find_injection;
+    (* repeat find_rewrite; *)
+    simpl in *; subst; intuition; 
+    eauto; try congruence);
+  repeat (
+    try (match goal with
+    | H1 : build_cvm (copland_compile ?t1) _ = _ 
+      |- _ =>
+        try (eapply IHt1 in H1)
+    | H2 : build_cvm (copland_compile ?t2) _ = _ 
+      |- _ =>
+        try (eapply IHt2 in H2)
+    end); 
+    try find_rewrite; eauto; 
+    try find_injection;
+    intuition; simpl in *; eauto
+  );
+  try (unfold remote_session, doRemote_session', do_remote in *;
+    monad_unfold; simpl in *; ff; eauto; fail);
+  try (
+    try (eapply IHt1 in Heqp; simpl in *);
+    try (eapply IHt1 in Heqp1; simpl in *);
+    try (eapply IHt1 in Heqp0; simpl in *);
+    try (eapply IHt2 in Heqp0; simpl in *);
+    try (eapply IHt2 in Heqp1; simpl in *);
+    find_rewrite; eauto).
+  - destruct a; 
+    repeat (try break_match; simpl in *; monad_unfold;
+      try find_injection; eauto).
+Qed.
+
+Definition supports_am (ac1 ac2 : AM_Config) : Prop :=
+  (forall aid l targ targid p' ev ev',
+      (forall res, 
+      ac1.(aspCb) (asp_paramsC aid l targ targid) p' ev ev' = resultC res ->
+      ac2.(aspCb) (asp_paramsC aid l targ targid) p' ev ev' = resultC res)) /\
+  (forall p, (forall res, 
+      ac1.(pubKeyCb) p = resultC res ->
+      ac2.(pubKeyCb) p = resultC res)) /\
+  (forall p, (forall res, 
+      ac1.(plcCb) p = resultC res ->
+      ac2.(plcCb) p = resultC res)) /\
+  (forall aid l targ targid p' ev ev',
+      ac1.(aspCb) (asp_paramsC aid l targ targid) p' ev ev' = errC Runtime ->
+      ac2.(aspCb) (asp_paramsC aid l targ targid) p' ev ev' = errC Runtime) /\
+  (forall p, 
+      ac1.(pubKeyCb) p = errC Runtime ->
+      ac2.(pubKeyCb) p = errC Runtime) /\
+  (forall p, 
+      ac1.(plcCb) p = errC Runtime ->
+      ac2.(plcCb) p = errC Runtime).
+
+Theorem supports_am_refl : forall ac1,
+  supports_am ac1 ac1.
+Proof.
+  unfold supports_am; intuition.
+Qed.
+
+Theorem supports_am_trans : forall ac1 ac2 ac3,
+  supports_am ac1 ac2 ->
+  supports_am ac2 ac3 ->
+  supports_am ac1 ac3.
+Proof.
+  unfold supports_am; intuition.
+Qed.
+
+Local Hint Resolve never_change_am_conf : core.
+Local Hint Resolve supports_am_refl : core.
+Local Hint Resolve supports_am_trans : core.
+
+Fixpoint am_config_support_exec (t : Term) 
+    (p : Plc) (ac : AM_Config) : Prop :=
+  match t with
+  | asp a =>
+      match a with
+      | NULL => True
+      | CPY => True
+      | SIG => 
+          forall l targ targid p' ev ev',
+          ((exists res, 
+          ac.(aspCb) (asp_paramsC sig_aspid l targ targid) p' ev ev' = resultC res) \/ 
+          ac.(aspCb) (asp_paramsC sig_aspid l targ targid) p' ev ev' = errC Runtime)
+      | HSH =>
+          forall l targ targid p' ev ev',
+          ((exists res, 
+          ac.(aspCb) (asp_paramsC hsh_aspid l targ targid) p' ev ev' = resultC res) \/ 
+          ac.(aspCb) (asp_paramsC hsh_aspid l targ targid) p' ev ev' = errC Runtime)
+      | ENC p =>
+          (forall l targ targid p' ev ev',
+          ((exists res, 
+          ac.(aspCb) (asp_paramsC enc_aspid l targ targid) p' ev ev' = resultC res) \/ 
+          ac.(aspCb) (asp_paramsC enc_aspid l targ targid) p' ev ev' = errC Runtime)) /\
+          ((exists res, ac.(pubKeyCb) p = resultC res) \/ 
+          ac.(pubKeyCb) p = errC Runtime)
+      | ASPC _ _ (asp_paramsC aspid _ _ _) =>
+          (forall l targ targid p' ev ev',
+          ((exists res, 
+          ac.(aspCb) (asp_paramsC aspid l targ targid) p' ev ev' = resultC res) \/ 
+          ac.(aspCb) (asp_paramsC aspid l targ targid) p' ev ev' = errC Runtime)) 
+      end
+  | att p' t' =>
+      ((exists res, ac.(plcCb) p' = resultC res) \/ 
+      ac.(plcCb) p' = errC Runtime)
+      (* /\ am_config_support_exec t' p' ac *)
+  | lseq t1 t2 =>
+      exists ac1 ac2,
+      (am_config_support_exec t1 p ac1) /\
+      (am_config_support_exec t2 p ac2) /\
+      supports_am ac1 ac /\
+      supports_am ac2 ac
+  | bseq _ t1 t2 =>
+      exists ac1 ac2,
+      (am_config_support_exec t1 p ac1) /\
+      (am_config_support_exec t2 p ac2) /\
+      supports_am ac1 ac /\
+      supports_am ac2 ac
+  | bpar _ t1 t2 =>
+      exists ac1 ac2,
+      (am_config_support_exec t1 p ac1) /\
+      (am_config_support_exec t2 p ac2) /\
+      supports_am ac1 ac /\
+      supports_am ac2 ac
+  end.
+
+Theorem well_formed_am_config_impl_executable : forall t p amConf,
+  am_config_support_exec t p amConf ->
+  forall st,
+  supports_am amConf (st.(st_AM_config)) ->
+  exists st', 
+    build_cvm (copland_compile t) st = (resultC tt, st') \/
+    build_cvm (copland_compile t) st = (errC (dispatch_error Runtime), st').
+Proof.
+  induction t; simpl in *; intuition; eauto.
+  - destruct a;
+    try (simpl in *; monad_unfold; eauto; fail); (* NULL, CPY *)
+    subst; simpl in *; try rewrite eqb_refl in *;
+    repeat (
+      try break_match;
+      try monad_unfold;
+      try break_match
+      try find_injection;
+      try find_contradiction;
+      try find_injection;
+      (* repeat find_rewrite; *)
+      simpl in *; subst; intuition; 
+      eauto; try congruence);
+    unfold supports_am, sig_params, enc_params, hsh_params in *; intuition;
+    match goal with
+    | H1 : forall _, _,
+      H2 : aspCb _ (asp_paramsC ?a ?l ?targ ?tid) ?p' ?ev ?ev' = _,
+      H3 : context[ aspCb _ _ _ _ _ = errC Runtime -> _],
+      H4 : context[ aspCb _ _ _ _ _ = resultC _ -> _]
+      |- _ =>
+        let H := fresh "H" in
+        let H' := fresh "Hx" in
+        let H'' := fresh "Hx" in
+        let res := fresh "res" in
+        destruct (H1 l targ tid p' ev ev') as [H | H]
+        ; 
+        [
+          (* result side *)
+          destruct H as [res H''];
+          pose proof (H4 a l targ tid p' ev ev') as H';
+          erewrite H' in *; eauto; congruence
+          |
+          (* err side *)
+          pose proof (H3 a l targ tid p' ev ev') as H';
+          intuition; find_rewrite; find_injection; eauto
+        ]
+    end.
+  - subst; simpl in *; try rewrite eqb_refl in *;
+    repeat (
+      unfold remote_session, doRemote_session', do_remote in *;
+      try break_match;
+      try monad_unfold;
+      try break_match
+      try find_injection;
+      try find_contradiction;
+      try find_injection;
+      (* repeat find_rewrite; *)
+      simpl in *; subst; intuition; 
+      eauto; try congruence);
+    unfold supports_am in *; intuition.
+    destruct H0;
+    erewrite H2 in *; try congruence; eauto.
+  - subst; simpl in *; try rewrite eqb_refl in *;
+    repeat (
+      unfold remote_session, doRemote_session', do_remote in *;
+      try break_match;
+      try monad_unfold;
+      try break_match
+      try find_injection;
+      try find_contradiction;
+      try find_injection;
+      (* repeat find_rewrite; *)
+      simpl in *; subst; intuition; 
+      eauto; try congruence);
+    unfold supports_am in *; intuition;
+    erewrite H6 in *; try congruence;
+    find_injection; eauto.
+  - subst; simpl in *; try rewrite eqb_refl in *;
+    repeat (
+      try break_match;
+      try monad_unfold;
+      try break_match
+      try find_injection;
+      try find_contradiction;
+      try find_injection;
+      (* repeat find_rewrite; *)
+      simpl in *; subst; intuition; 
+      eauto; try congruence);
+      match goal with
+      | H1 : exists _ _ : AM_Config, _
+        |- _ =>
+          let ac1 := fresh "ac" in
+          let ac2 := fresh "ac" in
+          let AS1 := fresh "AS" in
+          let AS2 := fresh "AS" in
+          let S1 := fresh "S" in
+          let S2 := fresh "S" in
+          destruct H1 as [ac1 [ac2 [AS1 [AS2 [S1 S2]]]]]
+          ;
+          match goal with
+          | H2 : build_cvm (copland_compile t1) ?st = _
+            |- _ =>
+              let A := fresh "A" in
+              assert (A : supports_am ac1 (st_AM_config st)); [ 
+                simpl in *; eauto
+                |
+                destruct (IHt1 p ac1 AS1 st A);
+                intuition; repeat find_rewrite;
+                repeat find_injection;
+                try congruence; eauto
+              ]
+          end;
+          match goal with
+          | H3 : build_cvm (copland_compile t2) ?st = _
+            |- _ =>
+              let A := fresh "A" in
+              assert (A : supports_am ac2 (st_AM_config st)); [ 
+                repeat find_eapply_lem_hyp never_change_am_conf;
+                repeat find_rewrite;
+                simpl in *; eauto
+                |
+                destruct (IHt2 p ac2 AS2 st A);
+                intuition; repeat find_rewrite;
+                repeat find_injection;
+                try congruence; eauto
+              ]
+          end
+      end. 
+  - subst; simpl in *; try rewrite eqb_refl in *;
+    repeat (
+      try break_match;
+      try monad_unfold;
+      try break_match
+      try find_injection;
+      try find_contradiction;
+      try find_injection;
+      (* repeat find_rewrite; *)
+      simpl in *; subst; intuition; 
+      eauto; try congruence);
+    match goal with
+    | H1 : exists _ _ : AM_Config, _
+      |- _ =>
+        let ac1 := fresh "ac" in
+        let ac2 := fresh "ac" in
+        let AS1 := fresh "AS" in
+        let AS2 := fresh "AS" in
+        let S1 := fresh "S" in
+        let S2 := fresh "S" in
+        destruct H1 as [ac1 [ac2 [AS1 [AS2 [S1 S2]]]]]
+        ;
+        match goal with
+        | H2 : build_cvm (copland_compile t1) ?st = _
+          |- _ =>
+            let A := fresh "A" in
+            assert (A : supports_am ac1 (st_AM_config st)); [ 
+              simpl in *; eauto
+              |
+              destruct (IHt1 p ac1 AS1 st A);
+              intuition; repeat find_rewrite;
+              repeat find_injection;
+              try congruence; eauto
+            ]
+        end;
+        match goal with
+        | H3 : build_cvm (copland_compile t2) ?st = _
+          |- _ =>
+            let A := fresh "A" in
+            assert (A : supports_am ac2 (st_AM_config st)); [ 
+              repeat find_eapply_lem_hyp never_change_am_conf;
+              repeat find_rewrite;
+              simpl in *; eauto
+              |
+              destruct (IHt2 p ac2 AS2 st A);
+              intuition; repeat find_rewrite;
+              repeat find_injection;
+              try congruence; eauto
+            ]
+        end;
+        repeat find_rewrite; eauto
+    end.
+  - subst; simpl in *; try rewrite eqb_refl in *;
+    repeat (
+      try break_match;
+      try monad_unfold;
+      try break_match
+      try find_injection;
+      try find_contradiction;
+      try find_injection;
+      (* repeat find_rewrite; *)
+      simpl in *; subst; intuition; 
+      eauto; try congruence);
+    match goal with
+    | H1 : exists _ _ : AM_Config, _
+      |- _ =>
+        let ac1 := fresh "ac" in
+        let ac2 := fresh "ac" in
+        let AS1 := fresh "AS" in
+        let AS2 := fresh "AS" in
+        let S1 := fresh "S" in
+        let S2 := fresh "S" in
+        destruct H1 as [ac1 [ac2 [AS1 [AS2 [S1 S2]]]]]
+        ;
+        match goal with
+        | H2 : build_cvm (copland_compile t1) ?st = _
+          |- _ =>
+            let A := fresh "A" in
+            assert (A : supports_am ac1 (st_AM_config st)); [ 
+              simpl in *; eauto
+              |
+              destruct (IHt1 p ac1 AS1 st A);
+              intuition; repeat find_rewrite;
+              repeat find_injection;
+              try congruence; eauto
+            ]
+        end;
+        match goal with
+        | H3 : build_cvm (copland_compile t2) ?st = _
+          |- _ =>
+            let A := fresh "A" in
+            assert (A : supports_am ac2 (st_AM_config st)); [ 
+              repeat find_eapply_lem_hyp never_change_am_conf;
+              repeat find_rewrite;
+              simpl in *; eauto
+              |
+              destruct (IHt2 p ac2 AS2 st A);
+              intuition; repeat find_rewrite;
+              repeat find_injection;
+              try congruence; eauto
+            ]
+        end;
+        repeat find_rewrite; eauto
+    end.
+  (* Unshelve. (* Weirdly, we have trivial existentials left *)
+  all: try (eapply default_bs); try (eapply default_UUID). *)
+Qed.
+
+Lemma in_add_to_list : forall {A} `{EqClass A} (l : list A) x x',
+  In x l ->
+  In x (add_to_list l x').
+Proof.
+  induction l; simpl in *; intuition; eauto;
+  subst; eauto; break_match; simpl in *; eauto.
+Qed.
+
+Local Hint Resolve in_add_to_list : core.
+
+
+(*
+
+Theorem generate_manifest'_preserves_plc : forall t p st st',
+  generate_manifest' t p st = st' ->
+  st.(my_abstract_plc) = st'.(my_abstract_plc).
+Proof.
+  induction t; simpl in *; intuition; eauto;
+  repeat break_match; subst; eauto;
+  try (destruct (generate_manifest' t1 p st) eqn:E1;
+    eapply IHt1 in E1; simpl in *;
+    destruct (generate_manifest' t2 p {|
+       my_abstract_plc := my_abstract_plc;
+       asps := asps;
+       uuidPlcs := uuidPlcs;
+       pubKeyPlcs := pubKeyPlcs;
+       targetPlcs := targetPlcs;
+       policy := policy
+     |}) eqn:E2;
+    eapply IHt2 in E2; simpl in *; subst; eauto).
+Qed.
+
+Theorem generate_manifest'_preserves_asps : forall t p st x st',
+  p = my_abstract_plc st ->
+  In x (asps st) ->
+  generate_manifest' t p st = st' ->
+  In x (asps st').
+Proof.
+  induction t; simpl in *; intuition; eauto;
+  subst; try rewrite eqb_refl in *; simpl in *;
+    repeat break_match; simpl in *;
+    try find_injection; eauto.
+  - destruct (generate_manifest' t1 (my_abstract_plc st) st) eqn:E1;
+    simpl in *.
+    eapply IHt1 in E1 as H'; eauto.
+    destruct (generate_manifest' t2 (Manifest.my_abstract_plc st) {|
+          my_abstract_plc := my_abstract_plc;
+          asps := asps;
+          uuidPlcs := uuidPlcs;
+          pubKeyPlcs := pubKeyPlcs;
+          targetPlcs := targetPlcs;
+          policy := policy
+        |}) eqn:E2; simpl in *; eauto.
+    eapply IHt2 in E2; eauto.
+    simpl in *.
+    eapply generate_manifest'_preserves_plc in E1;
+    eapply generate_manifest'_preserves_plc in E2;
+    simpl in *; subst; eauto.
+  - destruct (generate_manifest' t1 (my_abstract_plc st) st) eqn:E1;
+    simpl in *.
+    eapply IHt1 in E1 as H'; eauto.
+    destruct (generate_manifest' t2 (Manifest.my_abstract_plc st) {|
+          my_abstract_plc := my_abstract_plc;
+          asps := asps;
+          uuidPlcs := uuidPlcs;
+          pubKeyPlcs := pubKeyPlcs;
+          targetPlcs := targetPlcs;
+          policy := policy
+        |}) eqn:E2; simpl in *; eauto.
+    eapply IHt2 in E2; eauto.
+    simpl in *.
+    eapply generate_manifest'_preserves_plc in E1;
+    eapply generate_manifest'_preserves_plc in E2;
+    simpl in *; subst; eauto.
+  - destruct (generate_manifest' t1 (my_abstract_plc st) st) eqn:E1;
+    simpl in *.
+    eapply IHt1 in E1 as H'; eauto.
+    destruct (generate_manifest' t2 (Manifest.my_abstract_plc st) {|
+          my_abstract_plc := my_abstract_plc;
+          asps := asps;
+          uuidPlcs := uuidPlcs;
+          pubKeyPlcs := pubKeyPlcs;
+          targetPlcs := targetPlcs;
+          policy := policy
+        |}) eqn:E2; simpl in *; eauto.
+    eapply IHt2 in E2; eauto.
+    simpl in *.
+    eapply generate_manifest'_preserves_plc in E1;
+    eapply generate_manifest'_preserves_plc in E2;
+    simpl in *; subst; eauto.
+Qed.
+
+Theorem generate_manifest'_preserves_pubKeyPlcs : forall t p st x st',
+  p = my_abstract_plc st ->
+  In x (pubKeyPlcs st) ->
+  generate_manifest' t p st = st' ->
+  In x (pubKeyPlcs st').
+Proof.
+  induction t; simpl in *; intuition; eauto;
+  subst; try rewrite eqb_refl in *; simpl in *;
+    repeat break_match; simpl in *;
+    try find_injection; eauto.
+  - destruct (generate_manifest' t1 (my_abstract_plc st) st) eqn:E1;
+    simpl in *.
+    eapply IHt1 in E1 as H'; eauto.
+    destruct (generate_manifest' t2 (Manifest.my_abstract_plc st) {|
+          my_abstract_plc := my_abstract_plc;
+          asps := asps;
+          uuidPlcs := uuidPlcs;
+          pubKeyPlcs := pubKeyPlcs;
+          targetPlcs := targetPlcs;
+          policy := policy
+        |}) eqn:E2; simpl in *; eauto.
+    eapply IHt2 in E2; eauto.
+    simpl in *.
+    eapply generate_manifest'_preserves_plc in E1;
+    eapply generate_manifest'_preserves_plc in E2;
+    simpl in *; subst; eauto.
+  - destruct (generate_manifest' t1 (my_abstract_plc st) st) eqn:E1;
+    simpl in *.
+    eapply IHt1 in E1 as H'; eauto.
+    destruct (generate_manifest' t2 (Manifest.my_abstract_plc st) {|
+          my_abstract_plc := my_abstract_plc;
+          asps := asps;
+          uuidPlcs := uuidPlcs;
+          pubKeyPlcs := pubKeyPlcs;
+          targetPlcs := targetPlcs;
+          policy := policy
+        |}) eqn:E2; simpl in *; eauto.
+    eapply IHt2 in E2; eauto.
+    simpl in *.
+    eapply generate_manifest'_preserves_plc in E1;
+    eapply generate_manifest'_preserves_plc in E2;
+    simpl in *; subst; eauto.
+  - destruct (generate_manifest' t1 (my_abstract_plc st) st) eqn:E1;
+    simpl in *.
+    eapply IHt1 in E1 as H'; eauto.
+    destruct (generate_manifest' t2 (Manifest.my_abstract_plc st) {|
+          my_abstract_plc := my_abstract_plc;
+          asps := asps;
+          uuidPlcs := uuidPlcs;
+          pubKeyPlcs := pubKeyPlcs;
+          targetPlcs := targetPlcs;
+          policy := policy
+        |}) eqn:E2; simpl in *; eauto.
+    eapply IHt2 in E2; eauto.
+    simpl in *.
+    eapply generate_manifest'_preserves_plc in E1;
+    eapply generate_manifest'_preserves_plc in E2;
+    simpl in *; subst; eauto.
+Qed.
+
+
+Theorem generate_manifest'_preserves_uuidPlcs : forall t p st x st',
+  p = my_abstract_plc st ->
+  In x (uuidPlcs st) ->
+  generate_manifest' t p st = st' ->
+  In x (uuidPlcs st').
+Proof.
+  induction t; simpl in *; intuition; eauto;
+  subst; try rewrite eqb_refl in *; simpl in *;
+    repeat break_match; simpl in *;
+    try find_injection; eauto.
+  - destruct (generate_manifest' t1 (my_abstract_plc st) st) eqn:E1;
+    simpl in *.
+    eapply IHt1 in E1 as H'; eauto.
+    destruct (generate_manifest' t2 (Manifest.my_abstract_plc st) {|
+          my_abstract_plc := my_abstract_plc;
+          asps := asps;
+          uuidPlcs := uuidPlcs;
+          pubKeyPlcs := pubKeyPlcs;
+          targetPlcs := targetPlcs;
+          policy := policy
+        |}) eqn:E2; simpl in *; eauto.
+    eapply IHt2 in E2; eauto.
+    simpl in *.
+    eapply generate_manifest'_preserves_plc in E1;
+    eapply generate_manifest'_preserves_plc in E2;
+    simpl in *; subst; eauto.
+  - destruct (generate_manifest' t1 (my_abstract_plc st) st) eqn:E1;
+    simpl in *.
+    eapply IHt1 in E1 as H'; eauto.
+    destruct (generate_manifest' t2 (Manifest.my_abstract_plc st) {|
+          my_abstract_plc := my_abstract_plc;
+          asps := asps;
+          uuidPlcs := uuidPlcs;
+          pubKeyPlcs := pubKeyPlcs;
+          targetPlcs := targetPlcs;
+          policy := policy
+        |}) eqn:E2; simpl in *; eauto.
+    eapply IHt2 in E2; eauto.
+    simpl in *.
+    eapply generate_manifest'_preserves_plc in E1;
+    eapply generate_manifest'_preserves_plc in E2;
+    simpl in *; subst; eauto.
+  - destruct (generate_manifest' t1 (my_abstract_plc st) st) eqn:E1;
+    simpl in *.
+    eapply IHt1 in E1 as H'; eauto.
+    destruct (generate_manifest' t2 (Manifest.my_abstract_plc st) {|
+          my_abstract_plc := my_abstract_plc;
+          asps := asps;
+          uuidPlcs := uuidPlcs;
+          pubKeyPlcs := pubKeyPlcs;
+          targetPlcs := targetPlcs;
+          policy := policy
+        |}) eqn:E2; simpl in *; eauto.
+    eapply IHt2 in E2; eauto.
+    simpl in *.
+    eapply generate_manifest'_preserves_plc in E1;
+    eapply generate_manifest'_preserves_plc in E2;
+    simpl in *; subst; eauto.
+Qed.
+
+Local Hint Resolve generate_manifest'_preserves_asps : core.
+Local Hint Resolve generate_manifest'_preserves_plc : core.
+Local Hint Resolve generate_manifest'_preserves_pubKeyPlcs : core. 
+Local Hint Resolve generate_manifest'_preserves_uuidPlcs : core.
+
+Theorem lib_supports_cumul : 
+  forall t p st,
+  forall amLib absMan,
+  lib_supports_manifest amLib absMan ->
+  generate_manifest' t p st = absMan ->
+  lib_supports_manifest amLib st.
+Proof.
+  induction t; simpl in *; intuition; eauto;
+  try (repeat break_match; subst; eauto;
+  unfold lib_supports_manifest in *; intuition;
+  simpl in *; eauto; fail).
+Qed.
+*)
+
+Lemma in_add_to_list_rev : forall {A} `{EqClass A} (l : list A) (a a' : A),
+  a <> a' ->
+  In a (add_to_list l a') ->
+  In a l.
+Proof.
+  induction l; simpl in *; intuition; eauto.
+  break_match; simpl in *; intuition; eauto.
+Qed.
+
+Lemma in_dec_add_to_list : forall {A} `{EqClass A} l a a',
+  a <> a' ->
+  (if (in_dec (EqClass_impl_DecEq A) a l) then true else false) =  
+  if (in_dec (EqClass_impl_DecEq A) a (add_to_list l a')) then true else false.
+Proof.
+  intuition; repeat break_match; eauto.
+  - destruct n; eapply in_add_to_list; eauto.
+  - destruct n; eapply in_add_to_list_rev; eauto.
+Qed.
+
+Lemma cannot_be_in_filter_map : forall {A B} `{EqClass A} (l : MapC A B) l' a,
+  ~ (In a l') ->
+  map_get (minify_mapC l 
+    (fun x : A => if in_dec (EqClass_impl_DecEq A) x l' then true else false)) a = None.
+Proof.
+  induction l; simpl in *; intuition; eauto;
+  repeat (break_match; simpl in *; eauto; try congruence);
+  rewrite eqb_leibniz in *; congruence.
+Qed.
+
+Lemma cannot_be_in_filter_mapd : forall {A B} `{EqClass A, EqClass B} (l : MapD A B) l' a,
+  ~ (In a l') ->
+  map_get (minify_mapD l 
+    (fun x : A => if in_dec (EqClass_impl_DecEq A) x l' then true else false)) a = None.
+Proof.
+  induction l; simpl in *; intuition; eauto;
+  repeat (break_match; simpl in *; eauto; try congruence);
+  rewrite eqb_leibniz in *; congruence.
+Qed.
+
+Lemma map_get_minify_eq_under_add_to_list : forall {A B} `{EqClass A} (l : MapC A B) l' a a' v,
+  map_get (minify_mapC l 
+    (fun x : A => if in_dec (EqClass_impl_DecEq A) x l' then true else false)) a = Some v ->
+  map_get (minify_mapC l 
+    (fun x : A => if in_dec (EqClass_impl_DecEq A) x (add_to_list l' a') then true else false)) a = Some v.
+Proof.
+  induction l; simpl in *; intuition; eauto;
+  repeat (break_match; simpl in *; auto with *; eauto; try congruence);
+  rewrite eqb_leibniz in *; subst.
+  - assert (Some v = None). {
+      rewrite <- H0; eapply cannot_be_in_filter_map; eauto.
+    }
+    congruence.
+Qed.
+
+
+Lemma mapD_get_minify_eq_under_add_to_list : forall {A B} `{EqClass A, EqClass B} (l : MapD A B) l' a a' v,
+  map_get (minify_mapD l 
+    (fun x : A => if in_dec (EqClass_impl_DecEq A) x l' then true else false)) a = Some v ->
+  map_get (minify_mapD l 
+    (fun x : A => if in_dec (EqClass_impl_DecEq A) x (add_to_list l' a') then true else false)) a = Some v.
+Proof.
+  induction l; simpl in *; intuition; eauto;
+  repeat (break_match; simpl in *; auto with *; eauto; try congruence);
+  rewrite eqb_leibniz in *; subst.
+  - assert (Some v = None). {
+      rewrite <- H1; eapply cannot_be_in_filter_mapd; eauto.
+    }
+    congruence.
+Qed.
+
+(*
+
+Lemma man_comp_cumul : forall t p absMan amLib amConf absMan' amConf',
+  manifest_compiler absMan amLib = amConf ->
+  generate_manifest' t p absMan = absMan' ->
+  manifest_compiler absMan' amLib = amConf' ->
+  supports_am amConf amConf'.
+Proof.
+  induction t; try (simpl in *; intuition; eauto; fail).
+  - simpl in *; intuition; eauto;
+    destruct a; repeat break_match; simpl in *; subst; eauto;
+    rewrite eqb_leibniz in *; subst; eauto;
+    unfold supports_am in *; simpl in *; intuition; eauto;
+    unfold generate_PubKey_dispatcher in *; simpl in *; intuition; eauto;
+    repeat break_match; simpl in *; intuition; eauto; try congruence;
+    repeat find_injection; repeat find_rewrite; eauto; try congruence;
+    try (
+      try match goal with
+      | H1 : map_get (minify_mapC ?l 
+          (fun x : ASP_ID => 
+            if in_dec (EqClass_impl_DecEq ASP_ID) x ?l' then true else false)) ?a = ?res1,
+        H2 : map_get (minify_mapC ?l 
+          (fun x : ASP_ID => 
+            if in_dec (EqClass_impl_DecEq ASP_ID) x (add_to_list ?l' ?a') then true else false)) ?a = ?res2
+        |- _ =>
+          assert (res1 = res2) by (
+            eapply (map_get_minify_eq_under_add_to_list _ _ _ a') in H1;
+            rewrite <- H1, <- H2; eauto);
+          try find_injection; congruence
+      end;
+      match goal with
+      | H1 : map_get (minify_mapD ?l 
+          (fun x : _ => 
+            if in_dec (EqClass_impl_DecEq _) x ?l' then true else false)) ?a = ?res1,
+        H2 : map_get (minify_mapD ?l 
+          (fun x : _ => 
+            if in_dec (EqClass_impl_DecEq _) x (add_to_list ?l' ?a') then true else false)) ?a = ?res2
+        |- _ =>
+          assert (res1 = res2) by (
+            eapply (mapD_get_minify_eq_under_add_to_list _ _ _ a') in H1;
+            rewrite <- H1, <- H2; eauto);
+          try find_injection; congruence
+      end
+    ).
+  - simpl in *; intuition; eauto; subst.
+    unfold supports_am; simpl in *; intuition; eauto;
+    unfold generate_Plc_dispatcher in *;
+    repeat (repeat break_match; simpl in *; subst; eauto; try congruence);
+    match goal with
+      | H1 : map_get (minify_mapD ?l 
+          (fun x : _ => 
+            if in_dec (EqClass_impl_DecEq _) x ?l' then true else false)) ?a = ?res1,
+        H2 : map_get (minify_mapD ?l 
+          (fun x : _ => 
+            if in_dec (EqClass_impl_DecEq _) x (add_to_list ?l' ?a') then true else false)) ?a = ?res2
+        |- _ =>
+          assert (res1 = res2) by (
+            eapply (mapD_get_minify_eq_under_add_to_list _ _ _ a') in H1;
+            rewrite <- H1, <- H2; eauto);
+          try find_injection; congruence
+    end.
+Qed.
+
+Theorem man_gen_comp_works : forall t p backMan absMan amLib,
+  lib_supports_manifest amLib backMan ->
+  p = backMan.(my_abstract_plc) ->
+  generate_manifest' t p backMan = absMan ->
+  (* forall amLib, *)
+  lib_supports_manifest amLib absMan ->
+  (forall amConf,
+    manifest_compiler absMan amLib = amConf ->
+    (forall amConf',
+      supports_am amConf amConf' ->
+      am_config_support_exec t p amConf'
+    )
+  ).
+Proof.
+  induction t; simpl in *; intros.
+  - rewrite H0 in *;
+    rewrite eqb_refl in *;
+    unfold lib_supports_manifest, manifest_compiler in *;
+    destruct amConf; find_injection; simpl in *;
+    repeat (
+      try unfold generate_PubKey_dispatcher in *;
+      repeat break_match; repeat find_injection;
+      simpl in *; intuition; eauto; try congruence
+    ).
+    * destruct amConf'; simpl in *;
+      unfold supports_am in *; intuition; simpl in *;
+      pose proof (H3 a1 l0 targ targid p' ev ev');
+      pose proof (H8 a1 l0 targ targid p' ev ev');
+      repeat break_match; simpl in *;
+      repeat find_injection;
+      simpl in *; intuition; eauto; try congruence;
+      match goal with
+      | H:  context[ map_get (minify_mapC ?l ?filt) ?a],
+        H1: forall a' : Plc, _ -> (exists x : _, map_get _ _ = Some x) |- _ => 
+        assert (CO : exists x, map_get (minify_mapC l filt) a = Some x)
+        ;
+          [
+          eapply filter_resolver; eauto;
+          repeat break_match; intuition; try congruence
+          | 
+          rewrite H in CO; destruct CO; congruence
+        ]
+      | H:  context[ map_get (minify_mapD ?l ?filt) ?a],
+        H1: forall a' : Plc, _ -> (exists x : _, map_get _ _ = Some x) |- _ => 
+        assert (CO : exists x, map_get (minify_mapD l filt) a = Some x)
+        ;
+          [
+          eapply filter_resolver_mapd; eauto;
+          repeat break_match; intuition; try congruence
+          | 
+          rewrite H in CO; destruct CO; congruence
+        ]
+      end.
+    * destruct amConf'; simpl in *;
+      unfold supports_am in *; intuition; simpl in *;
+      pose proof (H3 sig_aspid l targ targid p' ev ev');
+      pose proof (H8 sig_aspid l targ targid p' ev ev');
+      repeat break_match; simpl in *;
+      repeat find_injection;
+      simpl in *; intuition; eauto; try congruence;
+      match goal with
+      | H:  context[ map_get (minify_mapC ?l ?filt) ?a],
+        H1: forall a' : Plc, _ -> (exists x : _, map_get _ _ = Some x) |- _ => 
+        assert (CO : exists x, map_get (minify_mapC l filt) a = Some x)
+        ;
+          [
+          eapply filter_resolver; eauto;
+          repeat break_match; intuition; try congruence
+          | 
+          rewrite H in CO; destruct CO; congruence
+        ]
+      | H:  context[ map_get (minify_mapD ?l ?filt) ?a],
+        H1: forall a' : Plc, _ -> (exists x : _, map_get _ _ = Some x) |- _ => 
+        assert (CO : exists x, map_get (minify_mapD l filt) a = Some x)
+        ;
+          [
+          eapply filter_resolver_mapd; eauto;
+          repeat break_match; intuition; try congruence
+          | 
+          rewrite H in CO; destruct CO; congruence
+        ]
+      end.
+    * destruct amConf'; simpl in *;
+      unfold supports_am in *; intuition; simpl in *;
+      pose proof (H3 hsh_aspid l targ targid p' ev ev');
+      pose proof (H8 hsh_aspid l targ targid p' ev ev');
+      repeat break_match; simpl in *;
+      repeat find_injection;
+      simpl in *; intuition; eauto; try congruence;
+      match goal with
+      | H:  context[ map_get (minify_mapC ?l ?filt) ?a],
+        H1: forall a' : Plc, _ -> (exists x : _, map_get _ _ = Some x) |- _ => 
+        assert (CO : exists x, map_get (minify_mapC l filt) a = Some x)
+        ;
+          [
+          eapply filter_resolver; eauto;
+          repeat break_match; intuition; try congruence
+          | 
+          rewrite H in CO; destruct CO; congruence
+        ]
+      | H:  context[ map_get (minify_mapD ?l ?filt) ?a],
+        H1: forall a' : Plc, _ -> (exists x : _, map_get _ _ = Some x) |- _ => 
+        assert (CO : exists x, map_get (minify_mapD l filt) a = Some x)
+        ;
+          [
+          eapply filter_resolver_mapd; eauto;
+          repeat break_match; intuition; try congruence
+          | 
+          rewrite H in CO; destruct CO; congruence
+        ]
+      end.
+    * destruct amConf'; simpl in *;
+      unfold supports_am in *; intuition; simpl in *;
+      pose proof (H3 enc_aspid l targ targid p' ev ev');
+      pose proof (H8 enc_aspid l targ targid p' ev ev');
+      repeat break_match; simpl in *;
+      repeat find_injection;
+      simpl in *; intuition; eauto; try congruence;
+      match goal with
+      | H:  context[ map_get (minify_mapC ?l ?filt) ?a],
+        H1: forall a' : Plc, _ -> (exists x : _, map_get _ _ = Some x) |- _ => 
+        assert (CO : exists x, map_get (minify_mapC l filt) a = Some x)
+        ;
+          [
+          eapply filter_resolver; eauto;
+          repeat break_match; intuition; try congruence
+          | 
+          rewrite H in CO; destruct CO; congruence
+        ]
+      | H:  context[ map_get (minify_mapD ?l ?filt) ?a],
+        H1: forall a' : Plc, _ -> (exists x : _, map_get _ _ = Some x) |- _ => 
+        assert (CO : exists x, map_get (minify_mapD l filt) a = Some x)
+        ;
+          [
+          eapply filter_resolver_mapd; eauto;
+          repeat break_match; intuition; try congruence
+          | 
+          rewrite H in CO; destruct CO; congruence
+        ]
+      end.
+    * destruct amConf'; simpl in *;
+      unfold supports_am in *; intuition; simpl in *.
+      pose proof (H4 p);
+      pose proof (H9 p);
+      repeat break_match; simpl in *;
+      repeat find_injection;
+      simpl in *; intuition; eauto; try congruence;
+      match goal with
+      | H:  context[ map_get (minify_mapC ?l ?filt) ?a],
+        H1: forall a' : Plc, _ -> (exists x : _, map_get _ _ = Some x) |- _ => 
+        assert (CO : exists x, map_get (minify_mapC l filt) a = Some x)
+        ;
+          [
+          eapply filter_resolver; eauto;
+          repeat break_match; intuition; try congruence
+          | 
+          rewrite H in CO; destruct CO; congruence
+        ]
+      | H:  context[ map_get (minify_mapD ?l ?filt) ?a],
+        H1: forall a' : Plc, _ -> (exists x : _, map_get _ _ = Some x) |- _ => 
+        assert (CO : exists x, map_get (minify_mapD l filt) a = Some x)
+        ;
+          [
+          eapply filter_resolver_mapd; eauto;
+          repeat break_match; intuition; try congruence
+          | 
+          rewrite H in CO; destruct CO; congruence
+        ]
+      end.
+  - unfold lib_supports_manifest, manifest_compiler in *;
+    destruct amConf; find_injection; simpl in *;
+    unfold supports_am in *; intuition; simpl in *;
+    pose proof (H5 p);
+    pose proof (H11 p);
+    repeat (
+      try unfold generate_Plc_dispatcher in *;
+      repeat break_match; repeat find_injection;
+      simpl in *; intuition; eauto; try congruence
+    );
+    
+    try (match goal with
+    | H:  context[ map_get (minify_mapC ?l ?filt) ?a],
+      H1: forall a' : Plc, _ -> (exists x : _, map_get _ _ = Some x) |- _ => 
+      assert (CO : exists x, map_get (minify_mapC l filt) a = Some x)
+      ;
+        [
+        eapply filter_resolver; eauto;
+        repeat break_match; intuition; try congruence
+        | 
+        rewrite H in CO; destruct CO; congruence
+      ]
+    | H:  context[ map_get (minify_mapD ?l ?filt) ?a],
+      H1: forall a' : Plc, _ -> (exists x : _, map_get _ _ = Some x) |- _ => 
+      assert (CO : exists x, map_get (minify_mapD l filt) a = Some x)
+      ;
+        [
+        eapply filter_resolver_mapd; eauto;
+        repeat break_match; intuition; try congruence
+        | 
+        rewrite H in CO; destruct CO; congruence
+      ]
+    end).
+  - destruct (generate_manifest' t1 p backMan) eqn:E1.
+    assert (lib_supports_manifest amLib
+      {|
+        my_abstract_plc := my_abstract_plc;
+        asps := asps;
+        uuidPlcs := uuidPlcs;
+        pubKeyPlcs := pubKeyPlcs;
+        targetPlcs := targetPlcs;
+        policy := policy
+      |}). {
+        eapply lib_supports_cumul; eauto.
+    }
+    pose proof (IHt1 _ _ _ _ H H0 E1 H5).
+    destruct (manifest_compiler {|
+         my_abstract_plc := my_abstract_plc;
+         asps := asps;
+         uuidPlcs := uuidPlcs;
+         pubKeyPlcs := pubKeyPlcs;
+         targetPlcs := targetPlcs;
+         policy := policy
+       |} amLib) eqn:M1.
+    pose proof (H6 {| concMan := concMan; aspCb := aspCb; plcCb := plcCb; pubKeyCb := pubKeyCb; uuidCb := uuidCb |} eq_refl {| concMan := concMan; aspCb := aspCb; plcCb := plcCb; pubKeyCb := pubKeyCb; uuidCb := uuidCb |} (supports_am_refl _)).
+    clear H6.
+    pose proof (IHt2 p {|
+         my_abstract_plc := my_abstract_plc;
+         asps := asps;
+         uuidPlcs := uuidPlcs;
+         pubKeyPlcs := pubKeyPlcs;
+         targetPlcs := targetPlcs;
+         policy := policy
+       |} absMan amLib). intuition. simpl in *.
+    intuition.
+    assert (p = my_abstract_plc). {
+      pose proof (generate_manifest'_preserves_plc _ _ _ _ E1);
+      simpl in *. repeat find_rewrite. eauto.
+    }
+    intuition.
+    pose proof (H9 _ H3 amConf'). intuition.
+    exists ({| concMan := concMan; aspCb := aspCb; plcCb := plcCb; pubKeyCb := pubKeyCb; uuidCb := uuidCb |}), amConf';
+    intuition; eauto.
+    eapply supports_am_trans; [ | eapply H4].
+    eapply man_comp_cumul. eauto.
+    eapply H1; eauto.
+    eapply H3.
+  - destruct (generate_manifest' t1 p backMan) eqn:E1.
+    assert (lib_supports_manifest amLib
+      {|
+        my_abstract_plc := my_abstract_plc;
+        asps := asps;
+        uuidPlcs := uuidPlcs;
+        pubKeyPlcs := pubKeyPlcs;
+        targetPlcs := targetPlcs;
+        policy := policy
+      |}). {
+        eapply lib_supports_cumul; eauto.
+    }
+    pose proof (IHt1 _ _ _ _ H H0 E1 H5).
+    destruct (manifest_compiler {|
+         my_abstract_plc := my_abstract_plc;
+         asps := asps;
+         uuidPlcs := uuidPlcs;
+         pubKeyPlcs := pubKeyPlcs;
+         targetPlcs := targetPlcs;
+         policy := policy
+       |} amLib) eqn:M1.
+    pose proof (H6 {| concMan := concMan; aspCb := aspCb; plcCb := plcCb; pubKeyCb := pubKeyCb; uuidCb := uuidCb |} eq_refl {| concMan := concMan; aspCb := aspCb; plcCb := plcCb; pubKeyCb := pubKeyCb; uuidCb := uuidCb |} (supports_am_refl _)).
+    clear H6.
+    pose proof (IHt2 p {|
+         my_abstract_plc := my_abstract_plc;
+         asps := asps;
+         uuidPlcs := uuidPlcs;
+         pubKeyPlcs := pubKeyPlcs;
+         targetPlcs := targetPlcs;
+         policy := policy
+       |} absMan amLib). intuition. simpl in *.
+    intuition.
+    assert (p = my_abstract_plc). {
+      pose proof (generate_manifest'_preserves_plc _ _ _ _ E1);
+      simpl in *. repeat find_rewrite. eauto.
+    }
+    intuition.
+    pose proof (H9 _ H3 amConf'). intuition.
+    exists ({| concMan := concMan; aspCb := aspCb; plcCb := plcCb; pubKeyCb := pubKeyCb; uuidCb := uuidCb |}), amConf';
+    intuition; eauto.
+    eapply supports_am_trans; [ | eapply H4].
+    eapply man_comp_cumul. eauto.
+    eapply H1; eauto.
+    eapply H3.
+  - destruct (generate_manifest' t1 p backMan) eqn:E1.
+    assert (lib_supports_manifest amLib
+      {|
+        my_abstract_plc := my_abstract_plc;
+        asps := asps;
+        uuidPlcs := uuidPlcs;
+        pubKeyPlcs := pubKeyPlcs;
+        targetPlcs := targetPlcs;
+        policy := policy
+      |}). {
+        eapply lib_supports_cumul; eauto.
+    }
+    pose proof (IHt1 _ _ _ _ H H0 E1 H5).
+    destruct (manifest_compiler {|
+         my_abstract_plc := my_abstract_plc;
+         asps := asps;
+         uuidPlcs := uuidPlcs;
+         pubKeyPlcs := pubKeyPlcs;
+         targetPlcs := targetPlcs;
+         policy := policy
+       |} amLib) eqn:M1.
+    pose proof (H6 {| concMan := concMan; aspCb := aspCb; plcCb := plcCb; pubKeyCb := pubKeyCb; uuidCb := uuidCb |} eq_refl {| concMan := concMan; aspCb := aspCb; plcCb := plcCb; pubKeyCb := pubKeyCb; uuidCb := uuidCb |} (supports_am_refl _)).
+    clear H6.
+    pose proof (IHt2 p {|
+         my_abstract_plc := my_abstract_plc;
+         asps := asps;
+         uuidPlcs := uuidPlcs;
+         pubKeyPlcs := pubKeyPlcs;
+         targetPlcs := targetPlcs;
+         policy := policy
+       |} absMan amLib). intuition. simpl in *.
+    intuition.
+    assert (p = my_abstract_plc). {
+      pose proof (generate_manifest'_preserves_plc _ _ _ _ E1);
+      simpl in *. repeat find_rewrite. eauto.
+    }
+    intuition.
+    pose proof (H9 _ H3 amConf'). intuition.
+    exists ({| concMan := concMan; aspCb := aspCb; plcCb := plcCb; pubKeyCb := pubKeyCb; uuidCb := uuidCb |}), amConf';
+    intuition; eauto.
+    eapply supports_am_trans; [ | eapply H4].
+    eapply man_comp_cumul. eauto.
+    eapply H1; eauto.
+    eapply H3.
+Qed.
+
+Theorem manifest_generator_compiler_soundess : forall t p absMan amLib amConf,
+  generate_manifest t p = absMan ->
+  lib_supports_manifest amLib absMan ->
+  manifest_compiler absMan amLib = amConf ->
+  forall st,
+    (* Note, this should be trivial typically as amConf = st.(st_AM_config) and refl works *)
+    supports_am amConf (st.(st_AM_config)) ->  
+    exists st', 
+      build_cvm (copland_compile t) st = (resultC tt, st') \/
+      build_cvm (copland_compile t) st = (errC (dispatch_error Runtime), st').
+Proof.
+  intros.
+  eapply well_formed_am_config_impl_executable.
+  - unfold generate_manifest in *; unfold empty_Manifest in *;
+    simpl in *;
+    assert (lib_supports_manifest amLib {| my_abstract_plc := p; asps := []; uuidPlcs := []; pubKeyPlcs := []; targetPlcs := []; policy := empty_PolicyT |}) by (unfold lib_supports_manifest; simpl in *; intuition; eauto);
+    assert (p = my_abstract_plc {| my_abstract_plc := p; asps := []; uuidPlcs := []; pubKeyPlcs := []; targetPlcs := []; policy := empty_PolicyT |}) by (simpl in *; eauto);
+    pose proof (man_gen_comp_works t _ _ _ _ H3 H4 H H0 _ H1); eauto.
+  - eapply supports_am_refl.
+Qed.
+
+*)
+
+Definition manifest_support_am_config (m : Manifest) (ac : AM_Config) : Prop :=
+  (forall a, In a (m.(asps)) -> 
+    forall l targ targid p' ev ev',
+    (exists res, ac.(aspCb) (asp_paramsC a l targ targid) p' ev ev' = resultC res) \/
+    (ac.(aspCb) (asp_paramsC a l targ targid) p' ev ev' = errC Runtime)) /\
+  (forall p, In p (m.(uuidPlcs)) ->
+    (exists res, ac.(plcCb) p = resultC res) \/
+    (ac.(plcCb) p = errC Runtime)) /\
+  (forall p, In p (m.(pubKeyPlcs)) ->
+    (exists res, ac.(pubKeyCb) p = resultC res) \/
+    (ac.(pubKeyCb) p = errC Runtime)).
+  
+(* 
+
+Theorem manifest_support_am_config_from_man_gen : forall t,
+  generate_manifest' t p backMan = absMan ->
+
+  manifest_support_am_config absMan () *)
+
+Theorem manifest_support_am_config_compiler : forall absMan amLib,
+  lib_supports_manifest amLib absMan ->
+  manifest_support_am_config absMan (manifest_compiler absMan amLib).
+Proof.
+  unfold lib_supports_manifest, manifest_support_am_config, 
+    manifest_compiler, generate_PubKey_dispatcher, generate_Plc_dispatcher in *;
+  simpl in *; intuition;
+  repeat break_match; simpl in *; intuition; eauto;
+  match goal with
+  | H:  context[ map_get (minify_mapC ?l ?filt) ?a],
+    H1: forall a' : Plc, _ -> (exists x : _, map_get _ _ = Some x) |- _ => 
+    assert (CO : exists x, map_get (minify_mapC l filt) a = Some x)
+    ;
+      [
+      eapply filter_resolver; eauto;
+      repeat break_match; intuition; try congruence
+      | 
+      rewrite H in CO; destruct CO; congruence
+    ]
+  | H:  context[ map_get (minify_mapD ?l ?filt) ?a],
+    H1: forall a' : Plc, _ -> (exists x : _, map_get _ _ = Some x) |- _ => 
+    assert (CO : exists x, map_get (minify_mapD l filt) a = Some x)
+    ;
+      [
+      eapply filter_resolver_mapd; eauto;
+      repeat break_match; intuition; try congruence
+      | 
+      rewrite H in CO; destruct CO; congruence
+    ]
+  end.
+Qed.
+
+Fixpoint manifest_support_term (m : Manifest) (t : Term) : Prop :=
+  match t with
+  | asp a =>
+      match a with
+      | NULL => True
+      | CPY => True
+      | SIG => 
+          In sig_aspid (m.(asps))
+      | HSH =>
+          In hsh_aspid (m.(asps))
+      | ENC p =>
+          In enc_aspid (m.(asps)) /\
+          In p (m.(pubKeyPlcs))
+      | ASPC _ _ (asp_paramsC aspid _ _ _) =>
+          In aspid (m.(asps))
+      end
+  | att p' t' =>
+      In p' (m.(uuidPlcs))
+  | lseq t1 t2 =>
+      manifest_support_term m t1 /\
+      manifest_support_term m t2
+  | bseq _ t1 t2 =>
+      manifest_support_term m t1 /\
+      manifest_support_term m t2
+  | bpar _ t1 t2 =>
+      manifest_support_term m t1 /\
+      manifest_support_term m t2
+  end.
+
+Theorem manifest_support_am_config_impl_am_config: forall t p absMan amConf,
+  manifest_support_am_config absMan amConf ->
+  manifest_support_term absMan t ->
+  am_config_support_exec t p amConf.
+Proof.
+  induction t; simpl in *; intuition; eauto;
+  unfold manifest_support_am_config in *; intuition; eauto;
+  repeat (try break_match; simpl in *; intuition; eauto).
+  - pose proof (IHt1 p absMan amConf); 
+    pose proof (IHt2 p absMan amConf); intuition;
+    exists amConf, amConf; eauto.
+  - pose proof (IHt1 p absMan amConf); 
+    pose proof (IHt2 p absMan amConf); intuition;
+    exists amConf, amConf; eauto.
+  - pose proof (IHt1 p absMan amConf); 
+    pose proof (IHt2 p absMan amConf); intuition;
+    exists amConf, amConf; eauto.
+Qed.
+
+(*
+
+Lemma manifest_support_term_unfold : forall t p backMan t',
+  manifest_support_term backMan t ->
+  p = (my_abstract_plc backMan) ->
+  manifest_support_term (generate_manifest' t' p backMan) t.
+Proof.
+  induction t; simpl in *; intuition; eauto;
+  repeat break_match; simpl in *; intuition; eauto.
+Qed.
+
+Theorem man_gen_always_supports : forall t p backMan,
+  p = (my_abstract_plc backMan) ->
+  manifest_support_term (generate_manifest' t p backMan) t.
+Proof.
+  induction t; intuition; try (simpl in *; eauto; fail);
+  try (simpl in *; intuition; eauto; [
+    eapply manifest_support_term_unfold; eauto | ];
+    rewrite H; eauto).
+  - repeat (try break_match; simpl in *; try congruence; eauto);
+    try (subst; rewrite eqb_refl in *; congruence).
+Qed.
+
+(* This proof tries to instead leverage the manifest_support notions *)
+Theorem man_gen_soundness' : forall t p absMan amLib amConf,
+  generate_manifest t p = absMan ->
+  lib_supports_manifest amLib absMan ->
+  manifest_compiler absMan amLib = amConf ->
+  forall st,
+    (* Note, this should be trivial typically as amConf = st.(st_AM_config) and refl works *)
+    supports_am amConf (st.(st_AM_config)) ->  
+  exists st', 
+    build_cvm (copland_compile t) st = (resultC tt, st') \/
+    build_cvm (copland_compile t) st = (errC (dispatch_error Runtime), st').
+Proof.
+  intros.
+  eapply well_formed_am_config_impl_executable.
+  - unfold generate_manifest, empty_Manifest in *; simpl in *.
+    eapply manifest_support_am_config_impl_am_config.
+    * eapply manifest_support_am_config_compiler; eauto.
+    * (* NOTE: This is the important one, substitute proof of any manifest here *)
+      rewrite <- H; eapply man_gen_always_supports; simpl in *; eauto.
+  - rewrite H1; eauto.
+  Unshelve. eapply min_id_type.
+Qed.
+*)
+
+
+(*
+
+
+Lemma manifest_support_term_unfold_old' : forall t p backEnv t' absMan absMan',
+  map_get backEnv p = Some absMan ->
+  manifest_support_term absMan t ->
+  map_get (manifest_generator' p t' backEnv) p = Some absMan' ->
+  manifest_support_term absMan' t.
+Proof.
+  induction t; intuition.
+  - simpl in *;
+    repeat break_match; simpl in *; intuition; eauto;
+    eapply man_gen_self_map_getter in H;
+    destruct H; intuition; eauto;
+    find_rewrite; find_injection; eauto.
+  - simpl in *;
+    eapply man_gen_self_map_getter in H;
+    destruct H; intuition; eauto;
+    find_rewrite; find_injection; eauto.
+  - simpl in *; intuition; eauto.
+  - simpl in *; intuition; eauto.
+  - simpl in *; intuition; eauto.
+Qed.
+
+Theorem map_get_man_gen_self_never_none : forall p t backMan,
+  exists res, map_get (manifest_generator' p t backMan) p = Some res.
+Proof.
+  induction t; simpl in *; intuition; eauto.
+  - unf; repeat break_match; simpl in *; eauto; subst; try congruence;
+    try (rewrite mapC_get_works; eexists; intuition; eauto; congruence).
+  - unfold at_manifest_generator, manifest_update_env, knowsof_manifest_update in *.
+    pose proof (man_gen_map_getter t p0 p (let
+           '{|
+              my_abstract_plc := oldPlc;
+              asps := oldasps;
+              uuidPlcs := oldKnowsOf;
+              pubKeyPlcs := oldContext;
+              targetPlcs := oldTargets;
+              policy := oldPolicy
+            |} := match map_get backMan p with
+                  | Some mm => mm
+                  | None => empty_Manifest
+                  end in
+            {|
+              my_abstract_plc := oldPlc;
+              asps := oldasps;
+              uuidPlcs := p0 :: oldKnowsOf;
+              pubKeyPlcs := oldContext;
+              targetPlcs := oldTargets;
+              policy := oldPolicy
+            |}) backMan). destruct H; intuition; eauto.
+Qed.
+
+*)
+
+
+Lemma places_decomp: forall t1 t2 p tp,
+In p (places' t2 (places' t1 [])) -> 
+(In p (places tp t1) \/ 
+      In p (places tp t2)).
+Proof.
+intros.
+
+assert (In p (places' t2 []) \/ In p (places' t1 [])).
+{
+  assert (In p (places' t1 []) \/ (~ In p (places' t1 []))).
+  { 
+      apply In_dec_tplc.
+  }
+  door.
+  +
+    eauto.
+  +             
+    assert (In p (places' t2 [])).
+    {
+      eapply places_app_cumul.
+      apply H.
+      eassumption.
+    }
+    eauto.
+}
+door.
+right.
+unfold places.
+right.
+eauto.
+
+left.
+right.
+eauto.
+Qed.
+
+Lemma has_manifest_env_places_env_has_manifest' : forall t p tp m e,
+map_get (manifest_generator' tp t e) p = Some m ->
+(exists m', map_get e p = Some m') \/ 
+In p (places tp t).
+Proof.
+
+intros.
+generalizeEverythingElse t.
+induction t; intros.
+-
+  destruct a; ff.
+  +
+    unfold asp_manifest_generator in *.
+    unfold asp_manifest_update in *.
+    unfold manifest_update_env in *.
+    ff.
+    ++
+
+    destruct (eq_plc_dec tp p); try solve_by_inversion.
+    left.
+    eexists.
+    eapply mapC_get_distinct_keys_from_set.
+    eassumption.
+    eassumption. 
+
+    ++
+    destruct (eq_plc_dec tp p); try solve_by_inversion.
+    left.
+    eexists.
+    eapply mapC_get_distinct_keys_from_set.
+    eassumption.
+    eassumption.
+    +
+    unfold asp_manifest_generator in *.
+    unfold asp_manifest_update in *.
+    unfold manifest_update_env in *.
+    ff.
+    ++
+
+    destruct (eq_plc_dec tp p); try solve_by_inversion.
+    left.
+    eexists.
+    eapply mapC_get_distinct_keys_from_set.
+    eassumption.
+    eassumption. 
+
+    ++
+    destruct (eq_plc_dec tp p); try solve_by_inversion.
+    left.
+    eexists.
+    eapply mapC_get_distinct_keys_from_set.
+    eassumption.
+    eassumption.
+    +
+    unfold asp_manifest_generator in *.
+    unfold asp_manifest_update in *.
+    unfold manifest_update_env in *.
+    ff.
+    ++
+
+    destruct (eq_plc_dec tp p); try solve_by_inversion.
+    left.
+    eexists.
+    eapply mapC_get_distinct_keys_from_set.
+    eassumption.
+    eassumption. 
+
+    ++
+    destruct (eq_plc_dec tp p); try solve_by_inversion.
+    left.
+    eexists.
+    eapply mapC_get_distinct_keys_from_set.
+    eassumption.
+    eassumption.
+    +
+    unfold asp_manifest_generator in *.
+    unfold asp_manifest_update in *.
+    unfold manifest_update_env in *.
+    ff.
+    ++
+
+    destruct (eq_plc_dec tp p); try solve_by_inversion.
+    left.
+    eexists.
+    eapply mapC_get_distinct_keys_from_set.
+    eassumption.
+    eassumption. 
+
+    ++
+    destruct (eq_plc_dec tp p); try solve_by_inversion.
+    left.
+    eexists.
+    eapply mapC_get_distinct_keys_from_set.
+    eassumption.
+    eassumption.
+    +
+    unfold asp_manifest_generator in *.
+    unfold asp_manifest_update in *.
+    unfold manifest_update_env in *.
+    ff.
+    ++
+
+    destruct (eq_plc_dec tp p); try solve_by_inversion.
+    left.
+    eexists.
+    eapply mapC_get_distinct_keys_from_set.
+    eassumption.
+    eassumption. 
+
+    ++
+    destruct (eq_plc_dec tp p); try solve_by_inversion.
+    left.
+    eexists.
+    eapply mapC_get_distinct_keys_from_set.
+    eassumption.
+    eassumption.
+    +
+    unfold asp_manifest_generator in *.
+    unfold asp_manifest_update in *.
+    unfold manifest_update_env in *.
+    ff.
+    ++
+
+    destruct (eq_plc_dec tp p); try solve_by_inversion.
+    left.
+    eexists.
+    eapply mapC_get_distinct_keys_from_set.
+    eassumption.
+    eassumption. 
+
+    ++
+    destruct (eq_plc_dec tp p); try solve_by_inversion.
+    left.
+    eexists.
+    eapply mapC_get_distinct_keys_from_set.
+    eassumption.
+    eassumption.
+  -
+  unfold manifest_generator in H.
+  simpl in H.
+  unfold at_manifest_generator in *.
+  ff.
+  unfold manifest_generator in IHt.
+
+  destruct (eq_plc_dec tp p0); try solve_by_inversion.
+  destruct (eq_plc_dec p p0); try solve_by_inversion.
+
+  apply IHt in H.
+  door.
+  +
+    unfold manifest_update_env in *.
+    ff; try solve_by_inversion.
+    ++
+    unfold knowsof_manifest_update in *.
+    ff.
+    subst.
+    ff.
+    left.
+    eexists.
+    eapply mapC_get_distinct_keys_from_set.
+    apply n. 
+    eassumption.
+    ++
+    left. 
+    eexists.
+    eapply mapC_get_distinct_keys_from_set.
+    apply n. 
+    eassumption.
+  +
+    door; try solve_by_inversion.
+  - (* lseq case *)
+    ff.
+
+    find_apply_hyp_hyp.
+
+    door.
+    +
+      find_apply_hyp_hyp.
+      door.
+      ++
+      left.
+      eauto.
+      ++
+      right.
+      door; eauto.
+      right.
+      Check places_decomp.
+
+      eapply places'_cumul.
+      eassumption.
+    +
+      door.
+      ++
+      right.
+      eauto.
+      ++
+      right.
+      right.
+      eapply places_app_cumul.
+      eassumption.
+      unfold not in *.
+      intros.
+      solve_by_inversion.
+  -
+  ff.
+
+  find_apply_hyp_hyp.
+
+  door.
+  +
+    find_apply_hyp_hyp.
+    door.
+    ++
+    left.
+    eauto.
+    ++
+    right.
+    door; eauto.
+    right.
+    Check places_decomp.
+
+    eapply places'_cumul.
+    eassumption.
+  +
+    door.
+    ++
+    right.
+    eauto.
+    ++
+    right.
+    right.
+    eapply places_app_cumul.
+    eassumption.
+    unfold not in *.
+    intros.
+    solve_by_inversion.
+
+  -
+  ff.
+
+  find_apply_hyp_hyp.
+
+  door.
+  +
+    find_apply_hyp_hyp.
+    door.
+    ++
+    left.
+    eauto.
+    ++
+    right.
+    door; eauto.
+    right.
+    Check places_decomp.
+
+    eapply places'_cumul.
+    eassumption.
+  +
+    door.
+    ++
+    right.
+    eauto.
+    ++
+    right.
+    right.
+    eapply places_app_cumul.
+    eassumption.
+    unfold not in *.
+    intros.
+    solve_by_inversion.
+Qed.
+
+Lemma has_manifest_env_places_env_has_manifest : forall t p tp m,
+map_get (manifest_generator t tp) p = Some m ->
+In p (places tp t).
+Proof.
+  intros.
+  unfold manifest_generator in *.
+  apply has_manifest_env_places_env_has_manifest' in H.
+  destruct_conjs.
+  door; ff. 
+Qed.
+
+Lemma places_env_has_manifest : forall t p tp e,
+In p (places tp t) -> 
+exists m, 
+map_get (manifest_generator' tp t e) p = Some m.
+Proof.
+  intros.
+  generalizeEverythingElse t.
+  induction t; intros.
+  -
+    ff.
+    door; try solve_by_inversion.
+    subst.
+    destruct a; 
+    unfold asp_manifest_generator;
+    unfold asp_manifest_update;
+    unfold manifest_update_env;
+    ff;
+    eexists;
+    eapply mapC_get_works.
+
+  - (* at case *)
+
+    ff.
+    door; ff.
+    subst.
+    unfold at_manifest_generator.
+    unfold knowsof_manifest_update.
+    ff.
+    unfold manifest_update_env.
+    ff.
+    +
+      subst.
+
+      assert (Environment_subset 
+      (map_set e p0
+          {|
+            my_abstract_plc := my_abstract_plc;
+            asps := asps;
+            uuidPlcs := p :: uuidPlcs;
+            pubKeyPlcs := pubKeyPlcs;
+            targetPlcs := targetPlcs;
+            policy := policy
+          |})
+
+          (manifest_generator' p t
+       (map_set e p0
+          {|
+            my_abstract_plc := my_abstract_plc;
+            asps := asps;
+            uuidPlcs := p :: uuidPlcs;
+            pubKeyPlcs := pubKeyPlcs;
+            targetPlcs := targetPlcs;
+            policy := policy
+          |}))
+      
+      ).
+      {
+        eapply manifest_generator_cumul'.
+      }
+      unfold Environment_subset in *.
+
+
+      assert (
+        map_get
+      (map_set e p0
+         {|
+           my_abstract_plc := my_abstract_plc;
+           asps := asps;
+           uuidPlcs := p :: uuidPlcs;
+           pubKeyPlcs := pubKeyPlcs;
+           targetPlcs := targetPlcs;
+           policy := policy
+         |}) p0 = Some {|
+         my_abstract_plc := my_abstract_plc;
+         asps := asps;
+         uuidPlcs := p :: uuidPlcs;
+         pubKeyPlcs := pubKeyPlcs;
+         targetPlcs := targetPlcs;
+         policy := policy
+       |}
+      ).
+      {
+        eapply mapC_get_works.
+
+      }
+
+      specialize H with (m1 := {|
+        my_abstract_plc := my_abstract_plc;
+        asps := asps;
+        uuidPlcs := p :: uuidPlcs;
+        pubKeyPlcs := pubKeyPlcs;
+        targetPlcs := targetPlcs;
+        policy := policy
+      |}) (p := p0).
+      find_apply_hyp_hyp.
+      destruct_conjs.
+
+      exists H0.
+      eauto.
+
+
+      +
+
+      subst.
+
+      assert (Environment_subset 
+      (map_set e p0
+          {|
+            my_abstract_plc := my_abstract_plc;
+            asps := asps;
+            uuidPlcs := p :: uuidPlcs;
+            pubKeyPlcs := pubKeyPlcs;
+            targetPlcs := targetPlcs;
+            policy := policy
+          |})
+
+          (manifest_generator' p t
+       (map_set e p0
+          {|
+            my_abstract_plc := my_abstract_plc;
+            asps := asps;
+            uuidPlcs := p :: uuidPlcs;
+            pubKeyPlcs := pubKeyPlcs;
+            targetPlcs := targetPlcs;
+            policy := policy
+          |}))
+      
+      ).
+      {
+        eapply manifest_generator_cumul'.
+      }
+      unfold Environment_subset in *.
+
+
+      assert (
+        map_get
+      (map_set e p0
+         {|
+           my_abstract_plc := my_abstract_plc;
+           asps := asps;
+           uuidPlcs := p :: uuidPlcs;
+           pubKeyPlcs := pubKeyPlcs;
+           targetPlcs := targetPlcs;
+           policy := policy
+         |}) p0 = Some {|
+         my_abstract_plc := my_abstract_plc;
+         asps := asps;
+         uuidPlcs := p :: uuidPlcs;
+         pubKeyPlcs := pubKeyPlcs;
+         targetPlcs := targetPlcs;
+         policy := policy
+       |}
+      ).
+      {
+        eapply mapC_get_works.
+
+      }
+
+      specialize H with (m1 := {|
+        my_abstract_plc := my_abstract_plc;
+        asps := asps;
+        uuidPlcs := p :: uuidPlcs;
+        pubKeyPlcs := pubKeyPlcs;
+        targetPlcs := targetPlcs;
+        policy := policy
+      |}) (p := p0).
+      find_apply_hyp_hyp.
+      destruct_conjs.
+
+      exists H0.
+      eauto.
+
+    - (* lseq case *)
+      ff.
+      door; ff.
+
+
+
+
+      assert (In p (places tp t1) \/ 
+              In p (places tp t2)).
+              {
+                eapply places_decomp; eauto.
+              }
+      door.
+      +
+        assert (exists mm, 
+                map_get (manifest_generator' tp t1 e) p = Some mm).
+        {
+          eauto.
+        }
+        destruct_conjs.
+
+        assert (Environment_subset 
+        (manifest_generator' tp t1 e)
+        (manifest_generator' tp t2
+         (manifest_generator' tp t1 e))
+        ).
+        {
+          eapply manifest_generator_cumul'.
+        }
+
+        unfold Environment_subset in *.
+        specialize H3 with (m1:=H1) (p:=p).
+        find_apply_hyp_hyp.
+        destruct_conjs.
+        eexists.
+        eassumption.
+
+      +
+      eapply IHt2.
+      unfold places in H0.
+      invc H0.
+      eauto.
+      eauto.
+
+
+      - (* lseq case *)
+      ff.
+      door; ff.
+
+
+
+
+      assert (In p (places tp t1) \/ 
+              In p (places tp t2)).
+              {
+                eapply places_decomp; eauto.
+              }
+      door.
+      +
+        assert (exists mm, 
+                map_get (manifest_generator' tp t1 e) p = Some mm).
+        {
+          eauto.
+        }
+        destruct_conjs.
+
+        assert (Environment_subset 
+        (manifest_generator' tp t1 e)
+        (manifest_generator' tp t2
+         (manifest_generator' tp t1 e))
+        ).
+        {
+          eapply manifest_generator_cumul'.
+        }
+
+        unfold Environment_subset in *.
+        specialize H3 with (m1:=H1) (p:=p).
+        find_apply_hyp_hyp.
+        destruct_conjs.
+        eexists.
+        eassumption.
+
+      +
+      eapply IHt2.
+      unfold places in H0.
+      invc H0.
+      eauto.
+      eauto.
+
+
+
+      - (* lseq case *)
+      ff.
+      door; ff.
+
+
+
+
+      assert (In p (places tp t1) \/ 
+              In p (places tp t2)).
+              {
+                eapply places_decomp; eauto.
+              }
+      door.
+      +
+        assert (exists mm, 
+                map_get (manifest_generator' tp t1 e) p = Some mm).
+        {
+          eauto.
+        }
+        destruct_conjs.
+
+        assert (Environment_subset 
+        (manifest_generator' tp t1 e)
+        (manifest_generator' tp t2
+         (manifest_generator' tp t1 e))
+        ).
+        {
+          eapply manifest_generator_cumul'.
+        }
+
+        unfold Environment_subset in *.
+        specialize H3 with (m1:=H1) (p:=p).
+        find_apply_hyp_hyp.
+        destruct_conjs.
+        eexists.
+        eassumption.
+
+      +
+      eapply IHt2.
+      unfold places in H0.
+      invc H0.
+      eauto.
+      eauto.
+Qed.
+
+
+
+(* TODO:  this is likely not provable forall p ... 
+   TODO:  perhaps generalize to something like:  
+            forall p, In p ((places t1 tp) ++ places e) ?? *)
+Lemma asdf : forall t1 t2 tp p' absMan e,
+map_get (manifest_generator' tp t2 
+            (manifest_generator' tp t1 e)) p' = Some absMan -> 
+In p' (places tp t1) ->
+exists m', 
+map_get (manifest_generator' tp t1 e) p' = Some m' /\ 
+manifest_subset m' absMan.
+Proof.
+  intros.
+
+  assert (Environment_subset 
+          (manifest_generator' tp t1 e)
+          (manifest_generator' tp t2
+            (manifest_generator' tp t1 e))
+          
+  ).
+  {
+    eapply manifest_generator_cumul'.
+    (*
+    Lemma manifest_generator_cumul : forall t p e1 e2,
+    Environment_subset e1 e2 ->
+    Environment_subset e1 (manifest_generator' p t e2).
+Proof.
+    
+    *)
+  }
+
+  eapply places_env_has_manifest in H0.
+  destruct_conjs.
+
+  unfold Environment_subset in *.
+
+  specialize H1 with (m1 := H0) (p:=p').
+
+  assert (
+    exists m2 : Manifest,
+       map_get
+         (manifest_generator' tp t2
+            (manifest_generator' tp t1 e)) p' =
+       Some m2 /\ manifest_subset H0 m2
+  ).
+  {
+    eapply H1.
+    eassumption.
+  }
+
+  destruct_conjs.
+  exists H0.
+  split; eauto.
+  find_rewrite.
+  ff.
+Qed.
+
+Lemma asdf_easy : forall t1 t2 tp absMan e,
+map_get (manifest_generator' tp t2 
+            (manifest_generator' tp t1 e)) tp = Some absMan -> 
+            
+exists m', (* p', 
+In p' (places tp t1) /\
+*)
+map_get (manifest_generator' tp t1 e) tp = Some m' /\ 
+manifest_subset m' absMan.
+Proof.
+  intros.
+  eapply asdf.
+  eassumption.
+  ff.
+  eauto.
+Qed.
+
+Lemma manifest_supports_term_sub : forall m1 m2 t,
+manifest_subset m1 m2 ->
+manifest_support_term m1 t -> 
+manifest_support_term m2 t.
+Proof.
+  intros.
+  generalizeEverythingElse t.
+  induction t; intros.
+  - (* asp case *)
+    ff.
+    ff.
+    subst.
+    unfold manifest_subset in *.
+    destruct_conjs.
+    eauto.
+  - (* at case *)
+    ff.
+    unfold manifest_subset in *.
+    destruct_conjs.
+    eauto.
+  - (* lseq case *)
+    ff.
+    destruct_conjs.
+    split; eauto.
+  - (* bseq case *)
+    ff.
+    destruct_conjs.
+    split; eauto.
+  - (* bpar case *)
+    ff.
+    destruct_conjs.
+    split; eauto.
+Qed.
+
+Lemma env_subset_man_subset : forall e1 e2 p m m',
+Environment_subset e1 e2 -> 
+map_get e1 p = Some m -> 
+map_get e2 p = Some m' -> 
+manifest_subset m m'.
+Proof.
+  intros.
+  unfold Environment_subset in *.
+  specialize H with (m1:= m) (p:=p).
+  find_apply_hyp_hyp.
+  destruct_conjs.
+  find_rewrite.
+  ff.
+Qed.
+
+Lemma fdsa : forall e e2 p p0 m absMan,
+Environment_subset
+  (map_set e p0 m) 
+  (e2) -> 
+map_get e2 p0 = Some absMan -> 
+In p (uuidPlcs m) -> 
+In p (uuidPlcs absMan).
+Proof.
+  intros.
+  assert (map_get (map_set e p0 m) p0 = Some m).
+  {
+    eapply mapC_get_works; eauto.
+  }
+  assert (manifest_subset m absMan).
+  {
+    eapply env_subset_man_subset; eauto.
+  }
+
+  unfold manifest_subset in *.
+  destruct_conjs.
+  eauto.
+Qed.
+
+Theorem man_gen_old_always_supports : forall t t' tp p backMan absMan,
+  map_get (manifest_generator' tp t backMan) p = Some absMan ->
+  In p (places tp t) ->
+  In t' (place_terms t tp p) ->
+  manifest_support_term absMan t'.
+Proof.
+
+  induction t; intuition.
+  - repeat (try break_match; 
+      unfold asp_manifest_generator, manifest_update_env, knowsof_manifest_update,
+        aspid_manifest_update, update_manifest_policy_targ, pubkey_manifest_update in *;
+      subst; simpl in *; intuition; eauto; try congruence;
+      repeat find_rewrite;
+      repeat find_injection;
+      simpl in * );
+    try (rewrite mapC_get_works in *; simpl in *; repeat find_injection; simpl in *; intuition; eauto).
+
+
+  - (* at case *)
+  ff.
+
+  ff.
+  +
+    door; try solve_by_inversion.
+    subst.
+    ff.
+    unfold at_manifest_generator in *.
+    ff.
+    unfold manifest_update_env in *.
+    ff.
+    ++
+      unfold knowsof_manifest_update in *.
+      ff.
+      subst.
+      assert (tp = p0).
+      {
+        eapply eqb_eq_plc; eauto.
+      }
+      subst.
+
+      pose (manifest_generator_cumul' t p 
+              (map_set backMan p0
+              {|
+                my_abstract_plc := my_abstract_plc;
+                asps := asps;
+                uuidPlcs := p :: uuidPlcs;
+                pubKeyPlcs := pubKeyPlcs;
+                targetPlcs := targetPlcs;
+                policy := policy
+              |})).
+
+    eapply fdsa; eauto.
+    simpl.
+    eauto.
+
+    ++
+    assert (tp = p0).
+    {
+      eapply eqb_eq_plc; eauto.
+    }
+    subst.
+
+
+    pose (manifest_generator_cumul' t p 
+            ((map_set backMan p0
+              {|
+                my_abstract_plc := empty_Manifest_Plc;
+                asps := [];
+                uuidPlcs := [p];
+                pubKeyPlcs := [];
+                targetPlcs := [];
+                policy := empty_PolicyT
+              |}))).
+
+    eapply fdsa; eauto.
+    simpl.
+    eauto.
+  +
+    door; eauto.
+    subst.
+    rewrite eqb_plc_refl in *.
+    solve_by_inversion.
+
+  - (* lseq case *)
+
+  ff.
+  ff.
+  +
+  door; try solve_by_inversion.
+  subst.
+  ff.
+  assert (tp = p).
+  {
+    eapply eqb_eq_plc; eauto.
+  }
+  subst.
+
+
+
+  split.
+    ++
+
+    find_apply_lem_hyp asdf_easy.
+    destruct_conjs.
+
+    eapply manifest_supports_term_sub.
+    eassumption.
+
+
+    eapply IHt1.
+    eassumption.
+    eauto.
+    apply top_plc_refl.
+
+  ++
+  eapply IHt2.
+  eassumption.
+  eauto.
+  apply top_plc_refl.
+
+
+  + (* tp <> p *)
+    destruct H0.
+    ++
+      subst.
+      rewrite eqb_plc_refl in *.
+      solve_by_inversion.
+    ++
+      assert ((In t' (place_terms t1 tp p)) \/ (In t' (place_terms t2 tp p))).
+      {
+        eapply in_app_or; eauto.
+      }
+      clear H1.
+
+      destruct H2.
+      +++ (* In t' (place_terms t1 tp p) *)
+        assert (In p (places tp t1)).
+        {
+          apply in_plc_term.
+          eapply in_not_nil.
+          eassumption.
+        }
+          find_apply_lem_hyp asdf.
+          ++++
+            destruct_conjs.
+            eapply manifest_supports_term_sub.
+            eassumption.
+            eapply IHt1.
+            eassumption.
+            eauto.
+            eassumption.
+
+          ++++
+            right.
+            unfold places in *.
+            invc H2.
+            +++++
+              rewrite eqb_plc_refl in Heqb.
+              solve_by_inversion.
+            +++++
+              eauto.
+      +++ (* In t' (place_terms t2 tp p) *)
+        simpl.
+
+        assert (In p (places tp t2)).
+      {
+        apply in_plc_term.
+        eapply in_not_nil; eauto.
+      }
+
+        eapply IHt2.
+        ++++
+          eassumption.
+        ++++
+          right.
+          unfold places in H2.
+          eauto.
+          invc H2.
+            +++++
+              rewrite eqb_plc_refl in *.
+              solve_by_inversion.
+            +++++
+              eassumption.
+          ++++
+            eassumption.
+
+  - (* bseq case*) 
+
+  ff.
+  ff.
+  +
+  door; try solve_by_inversion.
+  subst.
+  ff.
+  assert (tp = p).
+  {
+    eapply eqb_eq_plc; eauto.
+  }
+  subst.
+
+  split.
+    ++
+      find_apply_lem_hyp asdf_easy.
+      destruct_conjs.
+  
+      eapply manifest_supports_term_sub.
+      eassumption.
+  
+  
+      eapply IHt1.
+      eassumption.
+      eauto.
+      apply top_plc_refl.
+
+    ++
+      eapply IHt2.
+      eassumption.
+      eauto.
+      apply top_plc_refl.
+
+  + (* tp <> p *)
+    destruct H0.
+    ++
+      subst.
+      rewrite eqb_plc_refl in *.
+      solve_by_inversion.
+    ++
+      assert ((In t' (place_terms t1 tp p)) \/ (In t' (place_terms t2 tp p))).
+      {
+        eapply in_app_or; eauto.
+      }
+      clear H1.
+    
+      destruct H2.
+      +++ (* In t' (place_terms t1 tp p) *)
+        assert (In p (places tp t1)).
+        {
+          apply in_plc_term.
+          eapply in_not_nil.
+          eassumption.
+        }
+          find_apply_lem_hyp asdf.
+          ++++
+            destruct_conjs.
+        
+            eapply manifest_supports_term_sub.
+            eassumption.
+            eapply IHt1.
+            eassumption.
+            eauto.
+            eassumption.
+      
+          ++++
+            right.
+            unfold places in *.
+            invc H2.
+            +++++
+              rewrite eqb_plc_refl in Heqb.
+              solve_by_inversion.
+            +++++
+              eauto.
+      +++ (* In t' (place_terms t2 tp p) *)
+        simpl.
+    
+        assert (In p (places tp t2)).
+      {
+        apply in_plc_term.
+        eapply in_not_nil; eauto.
+      }
+    
+        eapply IHt2.
+        ++++
+          eassumption.
+        ++++
+          right.
+          unfold places in H2.
+          eauto.
+          invc H2.
+          +++++
+            rewrite eqb_plc_refl in *.
+            solve_by_inversion.
+          +++++
+            eassumption.
+        ++++
+          eassumption.
+
+
+  - (* bpar case*) 
+
+  ff.
+  ff.
+  +
+  door; try solve_by_inversion.
+  subst.
+  ff.
+  assert (tp = p).
+  {
+    eapply eqb_eq_plc; eauto.
+  }
+  subst.
+
+  split.
+    ++
+      find_apply_lem_hyp asdf_easy.
+      destruct_conjs.
+  
+      eapply manifest_supports_term_sub.
+      eassumption.
+  
+  
+      eapply IHt1.
+      eassumption.
+      eauto.
+      apply top_plc_refl.
+
+    ++
+      eapply IHt2.
+      eassumption.
+      eauto.
+      apply top_plc_refl.
+
+  + (* tp <> p *)
+    destruct H0.
+    ++
+      subst.
+      rewrite eqb_plc_refl in *.
+      solve_by_inversion.
+    ++
+      assert ((In t' (place_terms t1 tp p)) \/ (In t' (place_terms t2 tp p))).
+      {
+        eapply in_app_or; eauto.
+      }
+      clear H1.
+    
+      destruct H2.
+      +++ (* In t' (place_terms t1 tp p) *)
+        assert (In p (places tp t1)).
+        {
+          apply in_plc_term.
+          eapply in_not_nil.
+          eassumption.
+        }
+          find_apply_lem_hyp asdf.
+          ++++
+            destruct_conjs.
+        
+            eapply manifest_supports_term_sub.
+            eassumption.
+            eapply IHt1.
+            eassumption.
+            eauto.
+            eassumption.
+      
+          ++++
+            right.
+            unfold places in *.
+            invc H2.
+            +++++
+              rewrite eqb_plc_refl in Heqb.
+              solve_by_inversion.
+            +++++
+              eauto.
+      +++ (* In t' (place_terms t2 tp p) *)
+        simpl.
+    
+        assert (In p (places tp t2)).
+      {
+        apply in_plc_term.
+        eapply in_not_nil; eauto.
+      }
+    
+        eapply IHt2.
+        ++++
+          eassumption.
+        ++++
+          right.
+          unfold places in H2.
+          eauto.
+          invc H2.
+          +++++
+            rewrite eqb_plc_refl in *.
+            solve_by_inversion.
+          +++++
+            eassumption.
+        ++++
+          eassumption.
+Qed.
+
+Theorem manifest_generator_compiler_soundness_distributed : forall t tp p absMan amLib amConf,
+  map_get (manifest_generator t tp) p = Some absMan ->
+  lib_supports_manifest amLib absMan ->
+  manifest_compiler absMan amLib = amConf ->
+  forall st,
+    (* Note, this should be trivial typically as amConf = st.(st_AM_config) and refl works *)
+    supports_am amConf (st.(st_AM_config)) ->  
+
+    (  forall t', 
+         In t' (place_terms t tp p) -> 
+         st.(st_pl) = p -> 
+        
+         exists st', 
+        
+        build_cvm (copland_compile t') st = (resultC tt, st') \/
+        build_cvm (copland_compile t') st = (errC (dispatch_error Runtime), st')
+    ).
+Proof.
+  intros.
+  assert (In p (places tp t)) by 
+            (eapply has_manifest_env_places_env_has_manifest; eauto).
+  eapply well_formed_am_config_impl_executable.
+  - unfold manifest_generator, e_empty in *; simpl in *.
+    eapply manifest_support_am_config_impl_am_config.
+    * eapply manifest_support_am_config_compiler; eauto.
+    * (* NOTE: This is the important one, substitute proof of any manifest here *)
+      eapply man_gen_old_always_supports.
+      eassumption.
+      door.
+      +
+        subst.
+        unfold places.
+        left.
+        eauto.
+      +
+        unfold places.
+        right.
+        eauto.
+      +
+        subst.
+        eassumption.
+  - 
+    find_rewrite; eauto.
+  Unshelve. eapply min_id_type.
+Qed.
